@prefix : <http://www.semanticweb.org/danielhadad/ontologies/2022/7/AgriCardDB#> .
@prefix owl: <http://www.w3.org/2002/07/owl#> .
@prefix rdf: <http://www.w3.org/1999/02/22-rdf-syntax-ns#> .
@prefix xml: <http://www.w3.org/XML/1998/namespace> .
@prefix xsd: <http://www.w3.org/2001/XMLSchema#> .
@prefix agdb: <http://www.semanticweb.org/danielhadad/ontologies/2022/7/AgriCardDB#> .
@prefix rdfs: <http://www.w3.org/2000/01/rdf-schema#> .
@base <http://www.semanticweb.org/danielhadad/ontologies/2022/7/AgriCardDB> .

<http://www.semanticweb.org/danielhadad/ontologies/2022/7/AgriCardDB> rdf:type owl:Ontology ;
                                                                       rdfs:comment "A semantic card database for the board game Agricola." .

#################################################################
#    Object Properties
#################################################################

###  http://www.semanticweb.org/danielhadad/ontologies/2022/7/AgriCardDB#altersActionSpace
agdb:altersActionSpace rdf:type owl:ObjectProperty ;
                       rdfs:comment "Many cards change the way that the player or their opponents interact with action spaces by altering the effect of using them." .


###  http://www.semanticweb.org/danielhadad/ontologies/2022/7/AgriCardDB#categorizedBy
agdb:categorizedBy rdf:type owl:ObjectProperty ;
                   rdfs:comment "In this model categories include strategies, activation requirements, effect similarity, and other broad taxonomic considerations." .


###  http://www.semanticweb.org/danielhadad/ontologies/2022/7/AgriCardDB#givesAction
agdb:givesAction rdf:type owl:ObjectProperty ;
                 rdfs:subPropertyOf agdb:givesActionOrEffect ;
                 rdfs:comment "An action space or a card is related to an action or actions if using the action space or the card gives the player the ability to take that action or actions." .


###  http://www.semanticweb.org/danielhadad/ontologies/2022/7/AgriCardDB#givesActionOrEffect
agdb:givesActionOrEffect rdf:type owl:ObjectProperty ;
                         rdfs:comment "Action spaces and card effects give the player the ability to perform an action or actions or to resolve certain effects." .


###  http://www.semanticweb.org/danielhadad/ontologies/2022/7/AgriCardDB#givesEffect
agdb:givesEffect rdf:type owl:ObjectProperty ;
                 rdfs:subPropertyOf agdb:givesActionOrEffect .


###  http://www.semanticweb.org/danielhadad/ontologies/2022/7/AgriCardDB#provides
agdb:provides rdf:type owl:ObjectProperty ;
              rdfs:comment "A catchall property that has some in-game item as its object." .


#################################################################
#    Classes
#################################################################

###  http://www.semanticweb.org/danielhadad/ontologies/2022/7/AgriCardDB#Action
agdb:Action rdf:type owl:Class ;
            rdfs:subClassOf agdb:ActionOrEffect ;
            owl:disjointWith agdb:Effect .


###  http://www.semanticweb.org/danielhadad/ontologies/2022/7/AgriCardDB#ActionOrEffect
agdb:ActionOrEffect rdf:type owl:Class ;
                    rdfs:comment "The actions made available to players through placing person tokens on action spaces and/or resolving played cards. Additionally, the effects of using certain cards. Card effects might produce similar results to taking actions, but these are technically different." .


###  http://www.semanticweb.org/danielhadad/ontologies/2022/7/AgriCardDB#ActionSpace
agdb:ActionSpace rdf:type owl:Class ;
                 rdfs:comment "The board spaces that players place their person tokens on during their turn. Each action space allows the player to take a specific set of one or two actions." .


###  http://www.semanticweb.org/danielhadad/ontologies/2022/7/AgriCardDB#Animal
agdb:Animal rdf:type owl:Class ;
            rdfs:subClassOf agdb:GoodsAndFood ;
            owl:disjointWith agdb:Resource .


###  http://www.semanticweb.org/danielhadad/ontologies/2022/7/AgriCardDB#Banlist
agdb:Banlist rdf:type owl:Class ;
             rdfs:subClassOf agdb:CardSet ;
             rdfs:comment "Cards that are frequently removed from their respective decks because they are deemed anti-competitive or create problematic and confusing rule interactions." .


###  http://www.semanticweb.org/danielhadad/ontologies/2022/7/AgriCardDB#BoardActionSpace
agdb:BoardActionSpace rdf:type owl:Class ;
                      rdfs:subClassOf agdb:ActionSpace ;
                      owl:disjointWith agdb:PlayerCountActionSpace ,
                                       agdb:RoundActionSpace ;
                      rdfs:comment "The actions spaces that are always available from the start of round 1 regardless of player count." .


###  http://www.semanticweb.org/danielhadad/ontologies/2022/7/AgriCardDB#BuildingResource
agdb:BuildingResource rdf:type owl:Class ;
                      rdfs:subClassOf agdb:Resource ;
                      owl:disjointWith agdb:Crop .


###  http://www.semanticweb.org/danielhadad/ontologies/2022/7/AgriCardDB#Card
agdb:Card rdf:type owl:Class ;
          rdfs:comment "The class of cards that can be added to a player's farm." .


###  http://www.semanticweb.org/danielhadad/ontologies/2022/7/AgriCardDB#CardSet
agdb:CardSet rdf:type owl:Class ;
             rdfs:comment "A class for various collections of cards, representing either officially published decks or player-selected collections from a variety of published decks." .


###  http://www.semanticweb.org/danielhadad/ontologies/2022/7/AgriCardDB#Crop
agdb:Crop rdf:type owl:Class ;
          rdfs:subClassOf agdb:Resource .


###  http://www.semanticweb.org/danielhadad/ontologies/2022/7/AgriCardDB#Deck
agdb:Deck rdf:type owl:Class ;
          rdfs:subClassOf agdb:CardSet ;
          owl:disjointWith agdb:PlayerCollection ;
          rdfs:comment "A collection of cards that has been officially published or unofficially recognized as a specific set by community consensus." .


###  http://www.semanticweb.org/danielhadad/ontologies/2022/7/AgriCardDB#Effect
agdb:Effect rdf:type owl:Class ;
            rdfs:subClassOf agdb:ActionOrEffect .


###  http://www.semanticweb.org/danielhadad/ontologies/2022/7/AgriCardDB#FarmyardSpace
agdb:FarmyardSpace rdf:type owl:Class ;
                   rdfs:comment "Individuals in this class represent the various ways that squares on a player's board can be configured." .


###  http://www.semanticweb.org/danielhadad/ontologies/2022/7/AgriCardDB#Field
agdb:Field rdf:type owl:Class ;
           rdfs:subClassOf agdb:FarmyardSpace .


###  http://www.semanticweb.org/danielhadad/ontologies/2022/7/AgriCardDB#GameMarker
agdb:GameMarker rdf:type owl:Class ;
                rdfs:comment "The various physical tokens (excluding room and field tiles) used in the game." .


###  http://www.semanticweb.org/danielhadad/ontologies/2022/7/AgriCardDB#GameVersion
agdb:GameVersion rdf:type owl:Class .


###  http://www.semanticweb.org/danielhadad/ontologies/2022/7/AgriCardDB#GoodsAndFood
agdb:GoodsAndFood rdf:type owl:Class ;
                  rdfs:subClassOf agdb:GameMarker ;
                  owl:disjointWith agdb:PlayerToken ;
                  rdfs:comment "Individuals in this class represent the tokens for animals, resources, and food. There are no quantity limits on these tokens. Note: in the revised version of the game, food also counts as a good." .


###  http://www.semanticweb.org/danielhadad/ontologies/2022/7/AgriCardDB#HarvestPhase
agdb:HarvestPhase rdf:type owl:Class ;
                  rdfs:subClassOf agdb:Phase ;
                  rdfs:comment "In rounds that end with a harvest, the game enters the harvest phase after the returning home phase is completed. The harvest is further sub-divided into three phases." .


###  http://www.semanticweb.org/danielhadad/ontologies/2022/7/AgriCardDB#Improvement
agdb:Improvement rdf:type owl:Class ;
                 rdfs:subClassOf agdb:Card ;
                 owl:disjointWith agdb:Occupation ;
                 rdfs:comment "The class of Improvements" .


###  http://www.semanticweb.org/danielhadad/ontologies/2022/7/AgriCardDB#MajorImp
agdb:MajorImp rdf:type owl:Class ;
              rdfs:subClassOf agdb:Improvement ;
              owl:disjointWith agdb:MinorImp ;
              rdfs:comment "The class of fixed, communal Major Improvements." .


###  http://www.semanticweb.org/danielhadad/ontologies/2022/7/AgriCardDB#MinorImp
agdb:MinorImp rdf:type owl:Class ;
              rdfs:subClassOf agdb:Improvement ;
              rdfs:comment "The class of Minor Improvements that are dealt into players' hands along with Occupations." .


###  http://www.semanticweb.org/danielhadad/ontologies/2022/7/AgriCardDB#Occupation
agdb:Occupation rdf:type owl:Class ;
                rdfs:subClassOf agdb:Card ;
                rdfs:comment "The class of Occupations that are dealt into players' hands alongside Minor Improvements." .


###  http://www.semanticweb.org/danielhadad/ontologies/2022/7/AgriCardDB#Phase
agdb:Phase rdf:type owl:Class ;
           rdfs:comment "Each round proceeds in phases. The phase order is Preparation, Work, ReturningHome, and Harvest (for rounds that end in a harvest)." .


###  http://www.semanticweb.org/danielhadad/ontologies/2022/7/AgriCardDB#PlayerCollection
agdb:PlayerCollection rdf:type owl:Class ;
                      rdfs:subClassOf agdb:CardSet ;
                      rdfs:comment "A collection of cards from various decks curated by a player or players. May change over time." .


###  http://www.semanticweb.org/danielhadad/ontologies/2022/7/AgriCardDB#PlayerCountActionSpace
agdb:PlayerCountActionSpace rdf:type owl:Class ;
                            rdfs:subClassOf agdb:ActionSpace ;
                            owl:disjointWith agdb:RoundActionSpace ;
                            rdfs:comment "The action spaces that are always available from the start of round 1, depending on the number of players in the game." .


###  http://www.semanticweb.org/danielhadad/ontologies/2022/7/AgriCardDB#PlayerToken
agdb:PlayerToken rdf:type owl:Class ;
                 rdfs:subClassOf agdb:GameMarker ;
                 rdfs:comment "The colored game pieces given to each player during game set up. These represent fixed quantities." .


###  http://www.semanticweb.org/danielhadad/ontologies/2022/7/AgriCardDB#PublishedDeck
agdb:PublishedDeck rdf:type owl:Class ;
                   rdfs:subClassOf agdb:Deck ;
                   owl:disjointWith agdb:UnofficialDeck ;
                   rdfs:comment "Individuals in this class represent decks that have been officially published." .


###  http://www.semanticweb.org/danielhadad/ontologies/2022/7/AgriCardDB#Resource
agdb:Resource rdf:type owl:Class ;
              rdfs:subClassOf agdb:GoodsAndFood .


###  http://www.semanticweb.org/danielhadad/ontologies/2022/7/AgriCardDB#Room
agdb:Room rdf:type owl:Class ;
          rdfs:subClassOf agdb:FarmyardSpace .


###  http://www.semanticweb.org/danielhadad/ontologies/2022/7/AgriCardDB#RoundActionSpace
agdb:RoundActionSpace rdf:type owl:Class ;
                      rdfs:subClassOf agdb:ActionSpace ;
                      rdfs:comment "The action spaces that become available as the game progresses from one round to the next." .


###  http://www.semanticweb.org/danielhadad/ontologies/2022/7/AgriCardDB#Stage1ActionSpace
agdb:Stage1ActionSpace rdf:type owl:Class ;
                       owl:equivalentClass [ rdf:type owl:Class ;
                                             owl:oneOf ( agdb:FencesSpace
                                                         agdb:MajorMinorSpace
                                                         agdb:SowBakeSpace
                                                         <http://www.semanticweb.org/danielhadad/ontologies/2022/7/AgriCardDB#1SheepSpace>
                                                       )
                                           ] ;
                       rdfs:subClassOf agdb:RoundActionSpace ;
                       rdfs:comment "The action spaces that become available at the start of rounds 1, 2, 3, and 4." .


###  http://www.semanticweb.org/danielhadad/ontologies/2022/7/AgriCardDB#Stage2ActionSpace
agdb:Stage2ActionSpace rdf:type owl:Class ;
                       owl:equivalentClass [ rdf:type owl:Class ;
                                             owl:oneOf ( agdb:FGSpace
                                                         agdb:RenoImpSpace
                                                         <http://www.semanticweb.org/danielhadad/ontologies/2022/7/AgriCardDB#1StoneStage2Space>
                                                       )
                                           ] ;
                       rdfs:subClassOf agdb:RoundActionSpace ;
                       rdfs:comment "The action spaces that become available at the start of rounds 5, 6, and 7." .


###  http://www.semanticweb.org/danielhadad/ontologies/2022/7/AgriCardDB#Stage3ActionSpace
agdb:Stage3ActionSpace rdf:type owl:Class ;
                       owl:equivalentClass [ rdf:type owl:Class ;
                                             owl:oneOf ( agdb:Take1VegSpace
                                                         <http://www.semanticweb.org/danielhadad/ontologies/2022/7/AgriCardDB#1BoarSpace>
                                                       )
                                           ] ;
                       rdfs:subClassOf agdb:RoundActionSpace ;
                       rdfs:comment "The action spaces that become available at the start of rounds 8 and 9." .


###  http://www.semanticweb.org/danielhadad/ontologies/2022/7/AgriCardDB#Stage4ActionSpace
agdb:Stage4ActionSpace rdf:type owl:Class ;
                       owl:equivalentClass [ rdf:type owl:Class ;
                                             owl:oneOf ( <http://www.semanticweb.org/danielhadad/ontologies/2022/7/AgriCardDB#1CowSpace>
                                                         <http://www.semanticweb.org/danielhadad/ontologies/2022/7/AgriCardDB#1StoneStage4Space>
                                                       )
                                           ] ;
                       rdfs:subClassOf agdb:RoundActionSpace ;
                       rdfs:comment "The action spaces that become available at the start of rounds 10 and 11." .


###  http://www.semanticweb.org/danielhadad/ontologies/2022/7/AgriCardDB#Stage5ActionSpace
agdb:Stage5ActionSpace rdf:type owl:Class ;
                       owl:equivalentClass [ rdf:type owl:Class ;
                                             owl:oneOf ( agdb:FGWithoutRoomSpace
                                                         agdb:PlowSowSpace
                                                       )
                                           ] ;
                       rdfs:subClassOf agdb:RoundActionSpace ;
                       rdfs:comment "The action spaces that become available at the start of rounds 12 and 13." .


###  http://www.semanticweb.org/danielhadad/ontologies/2022/7/AgriCardDB#Stage6ActionSpace
agdb:Stage6ActionSpace rdf:type owl:Class ;
                       owl:equivalentClass [ rdf:type owl:Class ;
                                             owl:oneOf ( agdb:RenoFenceSpace
                                                       )
                                           ] ;
                       rdfs:subClassOf agdb:RoundActionSpace ;
                       rdfs:comment "The action space that becomes available at the start of round 14." .


###  http://www.semanticweb.org/danielhadad/ontologies/2022/7/AgriCardDB#UnofficialDeck
agdb:UnofficialDeck rdf:type owl:Class ;
                    rdfs:subClassOf agdb:Deck ;
                    rdfs:comment "Individuals in this class represent decks that have not been officially published but are recognized by the play-agricola community as constituting a singular deck." .


###  http://www.semanticweb.org/danielhadad/ontologies/2022/7/AgriCardDB#1PlusOccupation
<http://www.semanticweb.org/danielhadad/ontologies/2022/7/AgriCardDB#1PlusOccupation> rdf:type owl:Class ;
                                                                                      rdfs:subClassOf agdb:Occupation .


###  http://www.semanticweb.org/danielhadad/ontologies/2022/7/AgriCardDB#3PlayerActionSpace
<http://www.semanticweb.org/danielhadad/ontologies/2022/7/AgriCardDB#3PlayerActionSpace> rdf:type owl:Class ;
                                                                                         rdfs:subClassOf agdb:PlayerCountActionSpace ;
                                                                                         rdfs:comment "The action spaces that are placed on the game board during set up for a 3 player game." .


###  http://www.semanticweb.org/danielhadad/ontologies/2022/7/AgriCardDB#3PlusOccupation
<http://www.semanticweb.org/danielhadad/ontologies/2022/7/AgriCardDB#3PlusOccupation> rdf:type owl:Class ;
                                                                                      rdfs:subClassOf agdb:Occupation .


###  http://www.semanticweb.org/danielhadad/ontologies/2022/7/AgriCardDB#4PlayerActionSpace
<http://www.semanticweb.org/danielhadad/ontologies/2022/7/AgriCardDB#4PlayerActionSpace> rdf:type owl:Class ;
                                                                                         rdfs:subClassOf agdb:PlayerCountActionSpace ;
                                                                                         rdfs:comment "The action spaces that are placed on the game board during set up for a 4 player game." .


###  http://www.semanticweb.org/danielhadad/ontologies/2022/7/AgriCardDB#4PlusOccupation
<http://www.semanticweb.org/danielhadad/ontologies/2022/7/AgriCardDB#4PlusOccupation> rdf:type owl:Class ;
                                                                                      rdfs:subClassOf agdb:Occupation .


###  http://www.semanticweb.org/danielhadad/ontologies/2022/7/AgriCardDB#5PlayerActionSpace
<http://www.semanticweb.org/danielhadad/ontologies/2022/7/AgriCardDB#5PlayerActionSpace> rdf:type owl:Class ;
                                                                                         rdfs:subClassOf agdb:PlayerCountActionSpace ;
                                                                                         rdfs:comment "The action spaces that are placed on the game board during set up for a 5 player game." .


#################################################################
#    Individuals
#################################################################

###  http://www.semanticweb.org/danielhadad/ontologies/2022/7/AgriCardDB#BakeAct
agdb:BakeAct rdf:type owl:NamedIndividual ,
                      agdb:Action .


###  http://www.semanticweb.org/danielhadad/ontologies/2022/7/AgriCardDB#BeggingCardMarker
agdb:BeggingCardMarker rdf:type owl:NamedIndividual ,
                                agdb:GameMarker ;
                       rdfs:comment "Whenever a player cannot adequately feed their family during a harvest, or via the effects of certain cards, a player must add a Begging Card to their farm. At the end of the game, each Begging Card is worth -3 points." .


###  http://www.semanticweb.org/danielhadad/ontologies/2022/7/AgriCardDB#BuildFencesAct
agdb:BuildFencesAct rdf:type owl:NamedIndividual ,
                             agdb:Action .


###  http://www.semanticweb.org/danielhadad/ontologies/2022/7/AgriCardDB#BuildRoomAct
agdb:BuildRoomAct rdf:type owl:NamedIndividual ,
                           agdb:Action .


###  http://www.semanticweb.org/danielhadad/ontologies/2022/7/AgriCardDB#BuildSpace
agdb:BuildSpace rdf:type owl:NamedIndividual ,
                         agdb:BoardActionSpace ;
                rdfs:label "Build Room(s) and/or Stable(s)" .


###  http://www.semanticweb.org/danielhadad/ontologies/2022/7/AgriCardDB#BuildStableAct
agdb:BuildStableAct rdf:type owl:NamedIndividual ,
                             agdb:Action .


###  http://www.semanticweb.org/danielhadad/ontologies/2022/7/AgriCardDB#Cattle
agdb:Cattle rdf:type owl:NamedIndividual ,
                     agdb:Animal .


###  http://www.semanticweb.org/danielhadad/ontologies/2022/7/AgriCardDB#CheapOccSpace
agdb:CheapOccSpace rdf:type owl:NamedIndividual ,
                            agdb:BoardActionSpace ;
                   rdfs:comment "A player's first occupation is free, each additional one costs 1 Food" ;
                   rdfs:label "1 Occupation" .


###  http://www.semanticweb.org/danielhadad/ontologies/2022/7/AgriCardDB#Clay
agdb:Clay rdf:type owl:NamedIndividual ,
                   agdb:BuildingResource .


###  http://www.semanticweb.org/danielhadad/ontologies/2022/7/AgriCardDB#ClayHutRoom
agdb:ClayHutRoom rdf:type owl:NamedIndividual ,
                          agdb:Room .


###  http://www.semanticweb.org/danielhadad/ontologies/2022/7/AgriCardDB#DLSpace
agdb:DLSpace rdf:type owl:NamedIndividual ,
                      agdb:BoardActionSpace ;
             rdfs:label "Day Laborer" .


###  http://www.semanticweb.org/danielhadad/ontologies/2022/7/AgriCardDB#E
agdb:E rdf:type owl:NamedIndividual ,
                agdb:PublishedDeck ;
       rdfs:label "E Deck" .


###  http://www.semanticweb.org/danielhadad/ontologies/2022/7/AgriCardDB#EmptyField
agdb:EmptyField rdf:type owl:NamedIndividual ,
                         agdb:Field .


###  http://www.semanticweb.org/danielhadad/ontologies/2022/7/AgriCardDB#ExpensiveOccSpace
agdb:ExpensiveOccSpace rdf:type owl:NamedIndividual ,
                                <http://www.semanticweb.org/danielhadad/ontologies/2022/7/AgriCardDB#4PlayerActionSpace> ;
                       rdfs:comment "A player's first and second Occupation cost 1 Food each. Each Occupation after that costs 2 Food." ;
                       rdfs:label "1 Occupation" .


###  http://www.semanticweb.org/danielhadad/ontologies/2022/7/AgriCardDB#FGAct
agdb:FGAct rdf:type owl:NamedIndividual ,
                    agdb:Action .


###  http://www.semanticweb.org/danielhadad/ontologies/2022/7/AgriCardDB#FGSpace
agdb:FGSpace rdf:type owl:NamedIndividual ,
                      agdb:Stage2ActionSpace ;
             rdfs:label "After Family Growth also 1 Minor Improvement" .


###  http://www.semanticweb.org/danielhadad/ontologies/2022/7/AgriCardDB#FGWithoutRoomAct
agdb:FGWithoutRoomAct rdf:type owl:NamedIndividual ,
                               agdb:Action .


###  http://www.semanticweb.org/danielhadad/ontologies/2022/7/AgriCardDB#FGWithoutRoomSpace
agdb:FGWithoutRoomSpace rdf:type owl:NamedIndividual ,
                                 agdb:Stage5ActionSpace ;
                        rdfs:label "Family Growth even without space in your home" .


###  http://www.semanticweb.org/danielhadad/ontologies/2022/7/AgriCardDB#Fence
agdb:Fence rdf:type owl:NamedIndividual ,
                    agdb:PlayerToken .


###  http://www.semanticweb.org/danielhadad/ontologies/2022/7/AgriCardDB#FencedStable
agdb:FencedStable rdf:type owl:NamedIndividual ,
                           agdb:FarmyardSpace .


###  http://www.semanticweb.org/danielhadad/ontologies/2022/7/AgriCardDB#FencesSpace
agdb:FencesSpace rdf:type owl:NamedIndividual ,
                          agdb:Stage1ActionSpace ;
                 rdfs:label "Fences" .


###  http://www.semanticweb.org/danielhadad/ontologies/2022/7/AgriCardDB#FishingSpace
agdb:FishingSpace rdf:type owl:NamedIndividual ,
                           agdb:BoardActionSpace ;
                  rdfs:label "Fishing" .


###  http://www.semanticweb.org/danielhadad/ontologies/2022/7/AgriCardDB#Food
agdb:Food rdf:type owl:NamedIndividual ,
                   agdb:GoodsAndFood .


###  http://www.semanticweb.org/danielhadad/ontologies/2022/7/AgriCardDB#Fr
agdb:Fr rdf:type owl:NamedIndividual ,
                 agdb:PublishedDeck ;
        rdfs:label "France Deck" .


###  http://www.semanticweb.org/danielhadad/ontologies/2022/7/AgriCardDB#G
agdb:G rdf:type owl:NamedIndividual ,
                agdb:PublishedDeck ;
       rdfs:label "Gamer Deck" .


###  http://www.semanticweb.org/danielhadad/ontologies/2022/7/AgriCardDB#G4
agdb:G4 rdf:type owl:NamedIndividual ,
                 agdb:UnofficialDeck .


###  http://www.semanticweb.org/danielhadad/ontologies/2022/7/AgriCardDB#G5
agdb:G5 rdf:type owl:NamedIndividual ,
                 agdb:UnofficialDeck .


###  http://www.semanticweb.org/danielhadad/ontologies/2022/7/AgriCardDB#G6
agdb:G6 rdf:type owl:NamedIndividual ,
                 agdb:UnofficialDeck .


###  http://www.semanticweb.org/danielhadad/ontologies/2022/7/AgriCardDB#G7
agdb:G7 rdf:type owl:NamedIndividual ,
                 agdb:UnofficialDeck .


###  http://www.semanticweb.org/danielhadad/ontologies/2022/7/AgriCardDB#Grain
agdb:Grain rdf:type owl:NamedIndividual ,
                    agdb:Crop .


###  http://www.semanticweb.org/danielhadad/ontologies/2022/7/AgriCardDB#GuestToken
agdb:GuestToken rdf:type owl:NamedIndividual ,
                         agdb:GameMarker ;
                rdfs:comment "A token representing a temporary person on a player's farm or the board." .


###  http://www.semanticweb.org/danielhadad/ontologies/2022/7/AgriCardDB#HarvestBreedingPhase
agdb:HarvestBreedingPhase rdf:type owl:NamedIndividual ,
                                   agdb:HarvestPhase ;
                          rdfs:comment "If a player has at least two animals of the same type, the animals breed to process a newborn animal. The newborn animal must be housed on the player's farm and cannot be converted to food during this phase." .


###  http://www.semanticweb.org/danielhadad/ontologies/2022/7/AgriCardDB#HarvestFeedingPhase
agdb:HarvestFeedingPhase rdf:type owl:NamedIndividual ,
                                  agdb:HarvestPhase ;
                         rdfs:comment "In this phase, players must pay an appropriate amount of Food in order to feed their families." .


###  http://www.semanticweb.org/danielhadad/ontologies/2022/7/AgriCardDB#HarvestFieldPhase
agdb:HarvestFieldPhase rdf:type owl:NamedIndividual ,
                                agdb:HarvestPhase ;
                       rdfs:comment "The first phase of a harvest. Many card effects resolve during this phase. Fields are harvested." .


###  http://www.semanticweb.org/danielhadad/ontologies/2022/7/AgriCardDB#I
agdb:I rdf:type owl:NamedIndividual ,
                agdb:PublishedDeck ;
       rdfs:label "I Deck" .


###  http://www.semanticweb.org/danielhadad/ontologies/2022/7/AgriCardDB#K
agdb:K rdf:type owl:NamedIndividual ,
                agdb:PublishedDeck ;
       rdfs:label "K Deck" .


###  http://www.semanticweb.org/danielhadad/ontologies/2022/7/AgriCardDB#MajorMinorSpace
agdb:MajorMinorSpace rdf:type owl:NamedIndividual ,
                              agdb:Stage1ActionSpace ;
                     rdfs:label "1 Major or Minor Improvement" .


###  http://www.semanticweb.org/danielhadad/ontologies/2022/7/AgriCardDB#OccOrFGSpace
agdb:OccOrFGSpace rdf:type owl:NamedIndividual ,
                           <http://www.semanticweb.org/danielhadad/ontologies/2022/7/AgriCardDB#5PlayerActionSpace> ;
                  rdfs:comment "A player's first and second Occupations cost 1 Food each. Each additional Occupation costs 2 Food" ;
                  rdfs:label "1 Occupation or, From Round 5, Family Growth" .


###  http://www.semanticweb.org/danielhadad/ontologies/2022/7/AgriCardDB#OriginalVersion
agdb:OriginalVersion rdf:type owl:NamedIndividual ,
                              agdb:GameVersion .


###  http://www.semanticweb.org/danielhadad/ontologies/2022/7/AgriCardDB#Pasture
agdb:Pasture rdf:type owl:NamedIndividual ,
                      agdb:FarmyardSpace .


###  http://www.semanticweb.org/danielhadad/ontologies/2022/7/AgriCardDB#Person
agdb:Person rdf:type owl:NamedIndividual ,
                     agdb:PlayerToken .


###  http://www.semanticweb.org/danielhadad/ontologies/2022/7/AgriCardDB#PlantedField
agdb:PlantedField rdf:type owl:NamedIndividual ,
                           agdb:Field .


###  http://www.semanticweb.org/danielhadad/ontologies/2022/7/AgriCardDB#PlayMajorMinorAct
agdb:PlayMajorMinorAct rdf:type owl:NamedIndividual ,
                                agdb:Action .


###  http://www.semanticweb.org/danielhadad/ontologies/2022/7/AgriCardDB#PlayMinorAct
agdb:PlayMinorAct rdf:type owl:NamedIndividual ,
                           agdb:Action .


###  http://www.semanticweb.org/danielhadad/ontologies/2022/7/AgriCardDB#PlayOccAct
agdb:PlayOccAct rdf:type owl:NamedIndividual ,
                         agdb:Action .


###  http://www.semanticweb.org/danielhadad/ontologies/2022/7/AgriCardDB#PlayedImprovement
agdb:PlayedImprovement rdf:type owl:NamedIndividual ,
                                agdb:FarmyardSpace .


###  http://www.semanticweb.org/danielhadad/ontologies/2022/7/AgriCardDB#PlayedOccupation
agdb:PlayedOccupation rdf:type owl:NamedIndividual ,
                               agdb:FarmyardSpace .


###  http://www.semanticweb.org/danielhadad/ontologies/2022/7/AgriCardDB#PlowAct
agdb:PlowAct rdf:type owl:NamedIndividual ,
                      agdb:Action .


###  http://www.semanticweb.org/danielhadad/ontologies/2022/7/AgriCardDB#PlowSowSpace
agdb:PlowSowSpace rdf:type owl:NamedIndividual ,
                           agdb:Stage5ActionSpace ;
                  rdfs:label "Plow 1 Field and/or Sow" .


###  http://www.semanticweb.org/danielhadad/ontologies/2022/7/AgriCardDB#PlowSpace
agdb:PlowSpace rdf:type owl:NamedIndividual ,
                        agdb:BoardActionSpace ;
               rdfs:label "Plow 1 Field" .


###  http://www.semanticweb.org/danielhadad/ontologies/2022/7/AgriCardDB#PreparationPhase
agdb:PreparationPhase rdf:type owl:NamedIndividual ,
                               agdb:Phase ;
                      rdfs:comment "The first phase of a round. The new round card is flipped face up and the appropriate items are added to the board." .


###  http://www.semanticweb.org/danielhadad/ontologies/2022/7/AgriCardDB#RSFSpace
agdb:RSFSpace rdf:type owl:NamedIndividual ,
                       <http://www.semanticweb.org/danielhadad/ontologies/2022/7/AgriCardDB#4PlayerActionSpace> ;
              rdfs:comment "Take 1 Reed, 1 Stone, and 1 Food" .


###  http://www.semanticweb.org/danielhadad/ontologies/2022/7/AgriCardDB#ReceiveAnimalEffect
agdb:ReceiveAnimalEffect rdf:type owl:NamedIndividual ,
                                  agdb:Effect .


###  http://www.semanticweb.org/danielhadad/ontologies/2022/7/AgriCardDB#ReceiveBREffect
agdb:ReceiveBREffect rdf:type owl:NamedIndividual ,
                              agdb:Effect .


###  http://www.semanticweb.org/danielhadad/ontologies/2022/7/AgriCardDB#ReceiveBoarEffect
agdb:ReceiveBoarEffect rdf:type owl:NamedIndividual ,
                                agdb:Effect .


###  http://www.semanticweb.org/danielhadad/ontologies/2022/7/AgriCardDB#ReceiveClayEffect
agdb:ReceiveClayEffect rdf:type owl:NamedIndividual ,
                                agdb:Effect .


###  http://www.semanticweb.org/danielhadad/ontologies/2022/7/AgriCardDB#ReceiveCowEffect
agdb:ReceiveCowEffect rdf:type owl:NamedIndividual ,
                               agdb:Effect .


###  http://www.semanticweb.org/danielhadad/ontologies/2022/7/AgriCardDB#ReceiveEffect
agdb:ReceiveEffect rdf:type owl:NamedIndividual ,
                            agdb:Effect .


###  http://www.semanticweb.org/danielhadad/ontologies/2022/7/AgriCardDB#ReceiveFenceEffect
agdb:ReceiveFenceEffect rdf:type owl:NamedIndividual ,
                                 agdb:Effect .


###  http://www.semanticweb.org/danielhadad/ontologies/2022/7/AgriCardDB#ReceiveFieldEffect
agdb:ReceiveFieldEffect rdf:type owl:NamedIndividual ,
                                 agdb:Effect .


###  http://www.semanticweb.org/danielhadad/ontologies/2022/7/AgriCardDB#ReceiveFoodEffect
agdb:ReceiveFoodEffect rdf:type owl:NamedIndividual ,
                                agdb:Effect .


###  http://www.semanticweb.org/danielhadad/ontologies/2022/7/AgriCardDB#ReceiveGoodEffect
agdb:ReceiveGoodEffect rdf:type owl:NamedIndividual ,
                                agdb:Effect .


###  http://www.semanticweb.org/danielhadad/ontologies/2022/7/AgriCardDB#ReceiveGrainEffect
agdb:ReceiveGrainEffect rdf:type owl:NamedIndividual ,
                                 agdb:Effect .


###  http://www.semanticweb.org/danielhadad/ontologies/2022/7/AgriCardDB#ReceiveReedEffect
agdb:ReceiveReedEffect rdf:type owl:NamedIndividual ,
                                agdb:Effect .


###  http://www.semanticweb.org/danielhadad/ontologies/2022/7/AgriCardDB#ReceiveResourceEffect
agdb:ReceiveResourceEffect rdf:type owl:NamedIndividual ,
                                    agdb:Effect .


###  http://www.semanticweb.org/danielhadad/ontologies/2022/7/AgriCardDB#ReceiveRoomEffect
agdb:ReceiveRoomEffect rdf:type owl:NamedIndividual ,
                                agdb:Effect .


###  http://www.semanticweb.org/danielhadad/ontologies/2022/7/AgriCardDB#ReceiveSheepEffect
agdb:ReceiveSheepEffect rdf:type owl:NamedIndividual ,
                                 agdb:Effect .


###  http://www.semanticweb.org/danielhadad/ontologies/2022/7/AgriCardDB#ReceiveStableEffect
agdb:ReceiveStableEffect rdf:type owl:NamedIndividual ,
                                  agdb:Effect .


###  http://www.semanticweb.org/danielhadad/ontologies/2022/7/AgriCardDB#ReceiveStoneEffect
agdb:ReceiveStoneEffect rdf:type owl:NamedIndividual ,
                                 agdb:Effect .


###  http://www.semanticweb.org/danielhadad/ontologies/2022/7/AgriCardDB#ReceiveVegEffect
agdb:ReceiveVegEffect rdf:type owl:NamedIndividual ,
                               agdb:Effect .


###  http://www.semanticweb.org/danielhadad/ontologies/2022/7/AgriCardDB#ReceiveWoodEffect
agdb:ReceiveWoodEffect rdf:type owl:NamedIndividual ,
                                agdb:Effect .


###  http://www.semanticweb.org/danielhadad/ontologies/2022/7/AgriCardDB#Reed
agdb:Reed rdf:type owl:NamedIndividual ,
                   agdb:BuildingResource .


###  http://www.semanticweb.org/danielhadad/ontologies/2022/7/AgriCardDB#RenoAct
agdb:RenoAct rdf:type owl:NamedIndividual ,
                      agdb:Action .


###  http://www.semanticweb.org/danielhadad/ontologies/2022/7/AgriCardDB#RenoFenceSpace
agdb:RenoFenceSpace rdf:type owl:NamedIndividual ,
                             agdb:Stage6ActionSpace ;
                    rdfs:label "After Renovation also Fences" .


###  http://www.semanticweb.org/danielhadad/ontologies/2022/7/AgriCardDB#RenoImpSpace
agdb:RenoImpSpace rdf:type owl:NamedIndividual ,
                           agdb:Stage2ActionSpace ;
                  rdfs:label "After Renovation also 1 Major or Minor Improvement" .


###  http://www.semanticweb.org/danielhadad/ontologies/2022/7/AgriCardDB#ReturningHomePhase
agdb:ReturningHomePhase rdf:type owl:NamedIndividual ,
                                 agdb:Phase ;
                        rdfs:comment "The clean-up phase before the end of the round (in rounds without a harvest) or the start of a harvest. Many card effects resolve during this phase. All players return their person tokens to their farms." .


###  http://www.semanticweb.org/danielhadad/ontologies/2022/7/AgriCardDB#RevisedVersion
agdb:RevisedVersion rdf:type owl:NamedIndividual ,
                             agdb:GameVersion .


###  http://www.semanticweb.org/danielhadad/ontologies/2022/7/AgriCardDB#SPAct
agdb:SPAct rdf:type owl:NamedIndividual ,
                    agdb:Action .


###  http://www.semanticweb.org/danielhadad/ontologies/2022/7/AgriCardDB#SPSpace
agdb:SPSpace rdf:type owl:NamedIndividual ,
                      agdb:BoardActionSpace ;
             rdfs:label "Starting Player and/or Minor Improvement" .


###  http://www.semanticweb.org/danielhadad/ontologies/2022/7/AgriCardDB#Sheep
agdb:Sheep rdf:type owl:NamedIndividual ,
                    agdb:Animal .


###  http://www.semanticweb.org/danielhadad/ontologies/2022/7/AgriCardDB#SowAct
agdb:SowAct rdf:type owl:NamedIndividual ,
                     agdb:Action .


###  http://www.semanticweb.org/danielhadad/ontologies/2022/7/AgriCardDB#SowBakeSpace
agdb:SowBakeSpace rdf:type owl:NamedIndividual ,
                           agdb:Stage1ActionSpace ;
                  rdfs:label "Sow and/or Bake Bread" .


###  http://www.semanticweb.org/danielhadad/ontologies/2022/7/AgriCardDB#Stable
agdb:Stable rdf:type owl:NamedIndividual ,
                     agdb:PlayerToken .


###  http://www.semanticweb.org/danielhadad/ontologies/2022/7/AgriCardDB#Stone
agdb:Stone rdf:type owl:NamedIndividual ,
                    agdb:BuildingResource .


###  http://www.semanticweb.org/danielhadad/ontologies/2022/7/AgriCardDB#StoneHouseRoom
agdb:StoneHouseRoom rdf:type owl:NamedIndividual ,
                             agdb:Room .


###  http://www.semanticweb.org/danielhadad/ontologies/2022/7/AgriCardDB#TPSpace
agdb:TPSpace rdf:type owl:NamedIndividual ,
                      <http://www.semanticweb.org/danielhadad/ontologies/2022/7/AgriCardDB#4PlayerActionSpace> ;
             rdfs:comment "Traveling Players" .


###  http://www.semanticweb.org/danielhadad/ontologies/2022/7/AgriCardDB#Take1VegSpace
agdb:Take1VegSpace rdf:type owl:NamedIndividual ,
                            agdb:Stage3ActionSpace ;
                   rdfs:label "Take 1 Vegetable" .


###  http://www.semanticweb.org/danielhadad/ontologies/2022/7/AgriCardDB#TakeAct
agdb:TakeAct rdf:type owl:NamedIndividual ,
                      agdb:Action .


###  http://www.semanticweb.org/danielhadad/ontologies/2022/7/AgriCardDB#TakeAnimalAct
agdb:TakeAnimalAct rdf:type owl:NamedIndividual ,
                            agdb:Action .


###  http://www.semanticweb.org/danielhadad/ontologies/2022/7/AgriCardDB#TakeBRAct
agdb:TakeBRAct rdf:type owl:NamedIndividual ,
                        agdb:Action .


###  http://www.semanticweb.org/danielhadad/ontologies/2022/7/AgriCardDB#TakeBoar
agdb:TakeBoar rdf:type owl:NamedIndividual ,
                       agdb:Action .


###  http://www.semanticweb.org/danielhadad/ontologies/2022/7/AgriCardDB#TakeClayAct
agdb:TakeClayAct rdf:type owl:NamedIndividual ,
                          agdb:Action .


###  http://www.semanticweb.org/danielhadad/ontologies/2022/7/AgriCardDB#TakeCowAct
agdb:TakeCowAct rdf:type owl:NamedIndividual ,
                         agdb:Action .


###  http://www.semanticweb.org/danielhadad/ontologies/2022/7/AgriCardDB#TakeFoodAct
agdb:TakeFoodAct rdf:type owl:NamedIndividual ,
                          agdb:Action .


###  http://www.semanticweb.org/danielhadad/ontologies/2022/7/AgriCardDB#TakeGoodAct
agdb:TakeGoodAct rdf:type owl:NamedIndividual .


###  http://www.semanticweb.org/danielhadad/ontologies/2022/7/AgriCardDB#TakeGrainAct
agdb:TakeGrainAct rdf:type owl:NamedIndividual ,
                           agdb:Action .


###  http://www.semanticweb.org/danielhadad/ontologies/2022/7/AgriCardDB#TakeGrainSpace
agdb:TakeGrainSpace rdf:type owl:NamedIndividual ,
                             agdb:BoardActionSpace ;
                    rdfs:label "Take 1 Grain" .


###  http://www.semanticweb.org/danielhadad/ontologies/2022/7/AgriCardDB#TakeReedAct
agdb:TakeReedAct rdf:type owl:NamedIndividual ,
                          agdb:Action .


###  http://www.semanticweb.org/danielhadad/ontologies/2022/7/AgriCardDB#TakeResourceAct
agdb:TakeResourceAct rdf:type owl:NamedIndividual ,
                              agdb:Action .


###  http://www.semanticweb.org/danielhadad/ontologies/2022/7/AgriCardDB#TakeSheepAct
agdb:TakeSheepAct rdf:type owl:NamedIndividual ,
                           agdb:Action .


###  http://www.semanticweb.org/danielhadad/ontologies/2022/7/AgriCardDB#TakeStoneAct
agdb:TakeStoneAct rdf:type owl:NamedIndividual ,
                           agdb:Action .


###  http://www.semanticweb.org/danielhadad/ontologies/2022/7/AgriCardDB#TakeVegAct
agdb:TakeVegAct rdf:type owl:NamedIndividual ,
                         agdb:Action .


###  http://www.semanticweb.org/danielhadad/ontologies/2022/7/AgriCardDB#TakeWoodAct
agdb:TakeWoodAct rdf:type owl:NamedIndividual ,
                          agdb:Action .


###  http://www.semanticweb.org/danielhadad/ontologies/2022/7/AgriCardDB#UnfencedStable
agdb:UnfencedStable rdf:type owl:NamedIndividual ,
                             agdb:FarmyardSpace .


###  http://www.semanticweb.org/danielhadad/ontologies/2022/7/AgriCardDB#UnusedFarmSpace
agdb:UnusedFarmSpace rdf:type owl:NamedIndividual ,
                              agdb:FarmyardSpace .


###  http://www.semanticweb.org/danielhadad/ontologies/2022/7/AgriCardDB#Vegetable
agdb:Vegetable rdf:type owl:NamedIndividual ,
                        agdb:Crop .


###  http://www.semanticweb.org/danielhadad/ontologies/2022/7/AgriCardDB#WildBoar
agdb:WildBoar rdf:type owl:NamedIndividual ,
                       agdb:Animal .


###  http://www.semanticweb.org/danielhadad/ontologies/2022/7/AgriCardDB#Wm
agdb:Wm rdf:type owl:NamedIndividual ,
                 agdb:PublishedDeck ;
        rdfs:label "World Championship Deck" .


###  http://www.semanticweb.org/danielhadad/ontologies/2022/7/AgriCardDB#Wood
agdb:Wood rdf:type owl:NamedIndividual ,
                   agdb:BuildingResource .


###  http://www.semanticweb.org/danielhadad/ontologies/2022/7/AgriCardDB#WoodHutRoom
agdb:WoodHutRoom rdf:type owl:NamedIndividual ,
                          agdb:Room .


###  http://www.semanticweb.org/danielhadad/ontologies/2022/7/AgriCardDB#WorkPhase
agdb:WorkPhase rdf:type owl:NamedIndividual ,
                        agdb:Phase ;
               rdfs:comment "The round phase in which players use action spaces by placing person and/or guest tokens. Ends when all players have placed all of their available person and guest tokens." .


###  http://www.semanticweb.org/danielhadad/ontologies/2022/7/AgriCardDB#1AnimalSpace
<http://www.semanticweb.org/danielhadad/ontologies/2022/7/AgriCardDB#1AnimalSpace> rdf:type owl:NamedIndividual ,
                                                                                            <http://www.semanticweb.org/danielhadad/ontologies/2022/7/AgriCardDB#5PlayerActionSpace> ;
                                                                                   rdfs:label "Take 1 Sheep and 1 Food or Take 1 Wild Boar or Pay 1 Food for 1 Cattle" .


###  http://www.semanticweb.org/danielhadad/ontologies/2022/7/AgriCardDB#1BoarSpace
<http://www.semanticweb.org/danielhadad/ontologies/2022/7/AgriCardDB#1BoarSpace> rdf:type owl:NamedIndividual ,
                                                                                          agdb:Stage3ActionSpace ;
                                                                                 rdfs:label "1 Wild Boar" .


###  http://www.semanticweb.org/danielhadad/ontologies/2022/7/AgriCardDB#1ClaySpace
<http://www.semanticweb.org/danielhadad/ontologies/2022/7/AgriCardDB#1ClaySpace> rdf:type owl:NamedIndividual ,
                                                                                          agdb:BoardActionSpace ;
                                                                                 rdfs:label "1 Clay" .


###  http://www.semanticweb.org/danielhadad/ontologies/2022/7/AgriCardDB#1CowSpace
<http://www.semanticweb.org/danielhadad/ontologies/2022/7/AgriCardDB#1CowSpace> rdf:type owl:NamedIndividual ,
                                                                                         agdb:Stage4ActionSpace ;
                                                                                rdfs:label "1 Cattle" .


###  http://www.semanticweb.org/danielhadad/ontologies/2022/7/AgriCardDB#1ReedSpace
<http://www.semanticweb.org/danielhadad/ontologies/2022/7/AgriCardDB#1ReedSpace> rdf:type owl:NamedIndividual ,
                                                                                          agdb:BoardActionSpace ;
                                                                                 rdfs:label "1 Reed" .


###  http://www.semanticweb.org/danielhadad/ontologies/2022/7/AgriCardDB#1ReedStoneWoodSpace
<http://www.semanticweb.org/danielhadad/ontologies/2022/7/AgriCardDB#1ReedStoneWoodSpace> rdf:type owl:NamedIndividual ,
                                                                                                   <http://www.semanticweb.org/danielhadad/ontologies/2022/7/AgriCardDB#5PlayerActionSpace> ;
                                                                                          rdfs:label "1 Reed. In addition, take 1 Stone and 1 Wood" .


###  http://www.semanticweb.org/danielhadad/ontologies/2022/7/AgriCardDB#1ResourceSpace
<http://www.semanticweb.org/danielhadad/ontologies/2022/7/AgriCardDB#1ResourceSpace> rdf:type owl:NamedIndividual ,
                                                                                              <http://www.semanticweb.org/danielhadad/ontologies/2022/7/AgriCardDB#3PlayerActionSpace> ;
                                                                                     rdfs:label "Take 1 Building Resource of your choice" .


###  http://www.semanticweb.org/danielhadad/ontologies/2022/7/AgriCardDB#1RoomOrTPSpace
<http://www.semanticweb.org/danielhadad/ontologies/2022/7/AgriCardDB#1RoomOrTPSpace> rdf:type owl:NamedIndividual ,
                                                                                              <http://www.semanticweb.org/danielhadad/ontologies/2022/7/AgriCardDB#5PlayerActionSpace> ;
                                                                                     rdfs:label "Build 1 Room or Traveling Players" .


###  http://www.semanticweb.org/danielhadad/ontologies/2022/7/AgriCardDB#1SheepSpace
<http://www.semanticweb.org/danielhadad/ontologies/2022/7/AgriCardDB#1SheepSpace> rdf:type owl:NamedIndividual ,
                                                                                           agdb:Stage1ActionSpace ;
                                                                                  rdfs:label "1 Sheep" .


###  http://www.semanticweb.org/danielhadad/ontologies/2022/7/AgriCardDB#1StoneStage2Space
<http://www.semanticweb.org/danielhadad/ontologies/2022/7/AgriCardDB#1StoneStage2Space> rdf:type owl:NamedIndividual ,
                                                                                                 agdb:Stage2ActionSpace ;
                                                                                        rdfs:label "1 Stone" .


###  http://www.semanticweb.org/danielhadad/ontologies/2022/7/AgriCardDB#1StoneStage4Space
<http://www.semanticweb.org/danielhadad/ontologies/2022/7/AgriCardDB#1StoneStage4Space> rdf:type owl:NamedIndividual ,
                                                                                                 agdb:Stage4ActionSpace ;
                                                                                        rdfs:label "1 Stone" .


###  http://www.semanticweb.org/danielhadad/ontologies/2022/7/AgriCardDB#1WoodSpace
<http://www.semanticweb.org/danielhadad/ontologies/2022/7/AgriCardDB#1WoodSpace> rdf:type owl:NamedIndividual ,
                                                                                          <http://www.semanticweb.org/danielhadad/ontologies/2022/7/AgriCardDB#4PlayerActionSpace> ;
                                                                                 rdfs:label "1 Wood" .


###  http://www.semanticweb.org/danielhadad/ontologies/2022/7/AgriCardDB#2ClaySpace
<http://www.semanticweb.org/danielhadad/ontologies/2022/7/AgriCardDB#2ClaySpace> rdf:type owl:NamedIndividual ,
                                                                                          <http://www.semanticweb.org/danielhadad/ontologies/2022/7/AgriCardDB#4PlayerActionSpace> ;
                                                                                 rdfs:label "2 Clay" .


###  http://www.semanticweb.org/danielhadad/ontologies/2022/7/AgriCardDB#2WoodSpace
<http://www.semanticweb.org/danielhadad/ontologies/2022/7/AgriCardDB#2WoodSpace> rdf:type owl:NamedIndividual ,
                                                                                          <http://www.semanticweb.org/danielhadad/ontologies/2022/7/AgriCardDB#4PlayerActionSpace> ;
                                                                                 rdfs:label "2 Wood" .


###  http://www.semanticweb.org/danielhadad/ontologies/2022/7/AgriCardDB#3ClaySpace
<http://www.semanticweb.org/danielhadad/ontologies/2022/7/AgriCardDB#3ClaySpace> rdf:type owl:NamedIndividual ,
                                                                                          <http://www.semanticweb.org/danielhadad/ontologies/2022/7/AgriCardDB#5PlayerActionSpace> ;
                                                                                 rdfs:label "3 Clay" .


###  http://www.semanticweb.org/danielhadad/ontologies/2022/7/AgriCardDB#3Player1ClaySpace
<http://www.semanticweb.org/danielhadad/ontologies/2022/7/AgriCardDB#3Player1ClaySpace> rdf:type owl:NamedIndividual ,
                                                                                                 <http://www.semanticweb.org/danielhadad/ontologies/2022/7/AgriCardDB#3PlayerActionSpace> ;
                                                                                        rdfs:label "1 Clay" .


###  http://www.semanticweb.org/danielhadad/ontologies/2022/7/AgriCardDB#3Player2WoodSpace
<http://www.semanticweb.org/danielhadad/ontologies/2022/7/AgriCardDB#3Player2WoodSpace> rdf:type owl:NamedIndividual ,
                                                                                                 <http://www.semanticweb.org/danielhadad/ontologies/2022/7/AgriCardDB#3PlayerActionSpace> ;
                                                                                        rdfs:label "2 Wood" .


###  http://www.semanticweb.org/danielhadad/ontologies/2022/7/AgriCardDB#3PlayerExpensiveOccSpace
<http://www.semanticweb.org/danielhadad/ontologies/2022/7/AgriCardDB#3PlayerExpensiveOccSpace> rdf:type owl:NamedIndividual ,
                                                                                                        <http://www.semanticweb.org/danielhadad/ontologies/2022/7/AgriCardDB#3PlayerActionSpace> ;
                                                                                               rdfs:comment "Costs 2 Food" ;
                                                                                               rdfs:label "1 Occupation" .


###  http://www.semanticweb.org/danielhadad/ontologies/2022/7/AgriCardDB#3WoodSpace
<http://www.semanticweb.org/danielhadad/ontologies/2022/7/AgriCardDB#3WoodSpace> rdf:type owl:NamedIndividual ,
                                                                                          agdb:BoardActionSpace ;
                                                                                 rdfs:label "3 Wood" .


###  http://www.semanticweb.org/danielhadad/ontologies/2022/7/AgriCardDB#4WoodSpace
<http://www.semanticweb.org/danielhadad/ontologies/2022/7/AgriCardDB#4WoodSpace> rdf:type owl:NamedIndividual ,
                                                                                          <http://www.semanticweb.org/danielhadad/ontologies/2022/7/AgriCardDB#5PlayerActionSpace> ;
                                                                                 rdfs:label "4 Wood" .


#################################################################
#    General axioms
#################################################################

[ rdf:type owl:AllDisjointClasses ;
  owl:members ( agdb:Stage1ActionSpace
                agdb:Stage2ActionSpace
                agdb:Stage3ActionSpace
                agdb:Stage4ActionSpace
                agdb:Stage5ActionSpace
                agdb:Stage6ActionSpace
              )
] .


[ rdf:type owl:AllDisjointClasses ;
  owl:members ( <http://www.semanticweb.org/danielhadad/ontologies/2022/7/AgriCardDB#1PlusOccupation>
                <http://www.semanticweb.org/danielhadad/ontologies/2022/7/AgriCardDB#3PlusOccupation>
                <http://www.semanticweb.org/danielhadad/ontologies/2022/7/AgriCardDB#4PlusOccupation>
              )
] .


[ rdf:type owl:AllDisjointClasses ;
  owl:members ( <http://www.semanticweb.org/danielhadad/ontologies/2022/7/AgriCardDB#3PlayerActionSpace>
                <http://www.semanticweb.org/danielhadad/ontologies/2022/7/AgriCardDB#4PlayerActionSpace>
                <http://www.semanticweb.org/danielhadad/ontologies/2022/7/AgriCardDB#5PlayerActionSpace>
              )
] .


###  Generated by the OWL API (version 4.5.9.2019-02-01T07:24:44Z) https://github.com/owlcs/owlapi
