@prefix : <http://www.semanticweb.org/danielhadad/AgriGame#> .
@prefix owl: <http://www.w3.org/2002/07/owl#> .
@prefix rdf: <http://www.w3.org/1999/02/22-rdf-syntax-ns#> .
@prefix xml: <http://www.w3.org/XML/1998/namespace> .
@prefix xsd: <http://www.w3.org/2001/XMLSchema#> .
@prefix rdfs: <http://www.w3.org/2000/01/rdf-schema#> .
@base <http://www.semanticweb.org/danielhadad/AgriGame> .

<http://www.semanticweb.org/danielhadad/AgriGame> rdf:type owl:Ontology ;
                                                                     rdfs:comment "A semantic card database for the board game Agricola." .

#################################################################
#    Object Properties
#################################################################

###  http://www.semanticweb.org/danielhadad/AgriGame#hasPublisher
<http://www.semanticweb.org/danielhadad/AgriGame#hasPublisher> rdf:type owl:ObjectProperty .


###  http://www.semanticweb.org/danielhadad/AgriGame#hasVersion
<http://www.semanticweb.org/danielhadad/AgriGame#hasVersion> rdf:type owl:ObjectProperty .


###  http://www.semanticweb.org/danielhadad/AgriGame#addsToFuture
:addsToFuture rdf:type owl:ObjectProperty ;
              rdfs:comment "Some cards have the effect of adding items to the start of future rounds." .


###  http://www.semanticweb.org/danielhadad/AgriGame#alters
:alters rdf:type owl:ObjectProperty ;
        rdfs:comment "Many cards change the way that the player or their opponents interact with action spaces by altering the effect of using them." .


###  http://www.semanticweb.org/danielhadad/AgriGame#categorizedBy
:categorizedBy rdf:type owl:ObjectProperty ;
               rdfs:comment "In this model categories include strategies, activation requirements, effect similarity, and other broad taxonomic considerations." .


###  http://www.semanticweb.org/danielhadad/AgriGame#costs
:costs rdf:type owl:ObjectProperty .


###  http://www.semanticweb.org/danielhadad/AgriGame#costsOptionally
:costsOptionally rdf:type owl:ObjectProperty .


###  http://www.semanticweb.org/danielhadad/AgriGame#counters
:counters rdf:type owl:ObjectProperty ;
          rdfs:comment "Some cards counter the strategy set up by an opponent. Often, by producing a passive benefit whenever an opponent uses an action space that their strategy relies on." .


###  http://www.semanticweb.org/danielhadad/AgriGame#givesAction
:givesAction rdf:type owl:ObjectProperty ;
             rdfs:subPropertyOf :givesActionOrEffect ;
             rdfs:comment "An action space or a card is related to an action or actions if using the action space or the card gives the player the ability to take that action or actions." .


###  http://www.semanticweb.org/danielhadad/AgriGame#givesActionOrEffect
:givesActionOrEffect rdf:type owl:ObjectProperty ;
                     rdfs:comment "Action spaces and card effects give the player the ability to perform an action or actions or to resolve certain effects." .


###  http://www.semanticweb.org/danielhadad/AgriGame#givesEffect
:givesEffect rdf:type owl:ObjectProperty ;
             rdfs:subPropertyOf :givesActionOrEffect .


###  http://www.semanticweb.org/danielhadad/AgriGame#hasAuthor
:hasAuthor rdf:type owl:ObjectProperty .


###  http://www.semanticweb.org/danielhadad/AgriGame#hasValue
:hasValue rdf:type owl:ObjectProperty .


###  http://www.semanticweb.org/danielhadad/AgriGame#mentions
:mentions rdf:type owl:ObjectProperty ;
          rdfs:comment "Some cards specifically name other cards in their interactions" .


###  http://www.semanticweb.org/danielhadad/AgriGame#occursIn
:occursIn rdf:type owl:ObjectProperty ;
          rdfs:comment "Many effects have specific phases in which their effects resolve." .


###  http://www.semanticweb.org/danielhadad/AgriGame#partOf
:partOf rdf:type owl:ObjectProperty ;
        rdfs:comment "Cards are parts of Card Sets and Game Versions" .


###  http://www.semanticweb.org/danielhadad/AgriGame#provides
:provides rdf:type owl:ObjectProperty ;
          rdfs:comment "A catchall property that has some in-game item as its object." .


###  http://www.semanticweb.org/danielhadad/AgriGame#requires
:requires rdf:type owl:ObjectProperty ;
          rdfs:comment "Some cards can only be activated when a player's farm meets certain conditions." .


#################################################################
#    Data properties
#################################################################

###  http://www.semanticweb.org/danielhadad/AgriGame#isBanned
<http://www.semanticweb.org/danielhadad/AgriGame#isBanned> rdf:type owl:DatatypeProperty ;
                                                                            rdfs:range xsd:boolean .


###  http://www.semanticweb.org/danielhadad/AgriGame#hasAmount
:hasAmount rdf:type owl:DatatypeProperty .


###  http://www.semanticweb.org/danielhadad/AgriGame#hasDeckID
:hasDeckID rdf:type owl:DatatypeProperty ;
           rdfs:range xsd:integer .


###  http://www.semanticweb.org/danielhadad/AgriGame#hasMinPlayerCount
:hasMinPlayerCount rdf:type owl:DatatypeProperty ;
                   rdfs:range xsd:nonNegativeInteger .


###  http://www.semanticweb.org/danielhadad/AgriGame#hasText
:hasText rdf:type owl:DatatypeProperty ;
         rdfs:range xsd:string .


###  http://www.semanticweb.org/danielhadad/AgriGame#worthVP
:worthVP rdf:type owl:DatatypeProperty ;
         rdfs:range xsd:integer .


#################################################################
#    Classes
#################################################################

###  http://www.semanticweb.org/danielhadad/ontologies/2022/7/Agri#GameAuthor
<http://www.semanticweb.org/danielhadad/AgriGameAuthor> rdf:type owl:Class .


###  http://www.semanticweb.org/danielhadad/AgriGame#Publisher
<http://www.semanticweb.org/danielhadad/AgriGame#Publisher> rdf:type owl:Class .


###  http://www.semanticweb.org/danielhadad/AgriGame#Action
:Action rdf:type owl:Class ;
        rdfs:subClassOf :ActionOrEffect ;
        owl:disjointWith :Effect .


###  http://www.semanticweb.org/danielhadad/AgriGame#ActionOrEffect
:ActionOrEffect rdf:type owl:Class ;
                rdfs:comment "The actions made available to players through placing person tokens on action spaces and/or resolving played cards. Additionally, the effects of using certain cards. Card effects might produce similar results to taking actions, but these are technically different." .


###  http://www.semanticweb.org/danielhadad/AgriGame#ActionSpace
:ActionSpace rdf:type owl:Class ;
             rdfs:comment "The board spaces that players place their person tokens on during their turn. Each action space allows the player to take a specific set of one or two actions." .


###  http://www.semanticweb.org/danielhadad/AgriGame#Animal
:Animal rdf:type owl:Class ;
        rdfs:subClassOf :GoodsAndFood ;
        owl:disjointWith :Resource .


###  http://www.semanticweb.org/danielhadad/AgriGame#Banlist
:Banlist rdf:type owl:Class ;
         rdfs:subClassOf :CardSet ;
         rdfs:comment "Cards that are frequently removed from their respective decks because they are deemed anti-competitive or create problematic and confusing rule interactions." .


###  http://www.semanticweb.org/danielhadad/AgriGame#BoardActionSpace
:BoardActionSpace rdf:type owl:Class ;
                  rdfs:subClassOf :ActionSpace ;
                  owl:disjointWith :PlayerCountActionSpace ,
                                   :RoundActionSpace ;
                  rdfs:comment "The actions spaces that are always available from the start of round 1 regardless of player count." .


###  http://www.semanticweb.org/danielhadad/AgriGame#BuildingResource
:BuildingResource rdf:type owl:Class ;
                  rdfs:subClassOf :Resource ;
                  owl:disjointWith :Crop .


###  http://www.semanticweb.org/danielhadad/AgriGame#Card
:Card rdf:type owl:Class ;
      rdfs:comment "The class of cards that can be added to a player's farm." .


###  http://www.semanticweb.org/danielhadad/AgriGame#CardCost
:CardCost rdf:type owl:Class .


###  http://www.semanticweb.org/danielhadad/AgriGame#CardSet
:CardSet rdf:type owl:Class ;
         rdfs:comment "A class for various collections of cards, representing either officially published decks or player-selected collections from a variety of published decks." .


###  http://www.semanticweb.org/danielhadad/AgriGame#Category
:Category rdf:type owl:Class .


###  http://www.semanticweb.org/danielhadad/AgriGame#Crop
:Crop rdf:type owl:Class ;
      rdfs:subClassOf :Resource .


###  http://www.semanticweb.org/danielhadad/AgriGame#Deck
:Deck rdf:type owl:Class ;
      rdfs:subClassOf :CardSet ;
      owl:disjointWith :PlayerCollection ;
      rdfs:comment "A collection of cards that has been officially published or unofficially recognized as a specific set by community consensus." .


###  http://www.semanticweb.org/danielhadad/AgriGame#Designation
:Designation rdf:type owl:Class ;
             rdfs:subClassOf :Category ;
             rdfs:comment "Category subclass reserved for groups that are explicitly referenced by other cards." .


###  http://www.semanticweb.org/danielhadad/AgriGame#Effect
:Effect rdf:type owl:Class ;
        rdfs:subClassOf :ActionOrEffect .


###  http://www.semanticweb.org/danielhadad/AgriGame#FarmyardSpace
:FarmyardSpace rdf:type owl:Class ;
               rdfs:comment "Individuals in this class represent the various ways that squares on a player's board can be configured." .


###  http://www.semanticweb.org/danielhadad/AgriGame#Field
:Field rdf:type owl:Class ;
       rdfs:subClassOf :FarmyardSpace .


###  http://www.semanticweb.org/danielhadad/AgriGame#GameMarker
:GameMarker rdf:type owl:Class ;
            rdfs:comment "The various physical tokens (excluding room and field tiles) used in the game." .


###  http://www.semanticweb.org/danielhadad/AgriGame#GameVersion
:GameVersion rdf:type owl:Class .


###  http://www.semanticweb.org/danielhadad/AgriGame#GoodsAndFood
:GoodsAndFood rdf:type owl:Class ;
              rdfs:subClassOf :GameMarker ;
              owl:disjointWith :PlayerToken ;
              rdfs:comment "Individuals in this class represent the tokens for animals, resources, and food. There are no quantity limits on these tokens. Note: in the revised version of the game, food also counts as a good." .


###  http://www.semanticweb.org/danielhadad/AgriGame#HarvestPhase
:HarvestPhase rdf:type owl:Class ;
              rdfs:subClassOf :Phase ;
              rdfs:comment "In rounds that end with a harvest, the game enters the harvest phase after the returning home phase is completed. The harvest is further sub-divided into three phases." .


###  http://www.semanticweb.org/danielhadad/AgriGame#Improvement
:Improvement rdf:type owl:Class ;
             rdfs:subClassOf :Card ;
             owl:disjointWith :Occupation ;
             rdfs:comment "The class of Improvements" .


###  http://www.semanticweb.org/danielhadad/AgriGame#MajorImp
:MajorImp rdf:type owl:Class ;
          rdfs:subClassOf :Improvement ;
          owl:disjointWith :MinorImp ;
          rdfs:comment "The class of fixed, communal Major Improvements." .


###  http://www.semanticweb.org/danielhadad/AgriGame#MinorImp
:MinorImp rdf:type owl:Class ;
          rdfs:subClassOf :Improvement ;
          rdfs:comment "The class of Minor Improvements that are dealt into players' hands along with Occupations." .


###  http://www.semanticweb.org/danielhadad/AgriGame#Occupation
:Occupation rdf:type owl:Class ;
            rdfs:subClassOf :Card ;
            rdfs:comment "The class of Occupations that are dealt into players' hands alongside Minor Improvements." .


###  http://www.semanticweb.org/danielhadad/AgriGame#Phase
:Phase rdf:type owl:Class ;
       rdfs:comment "Each round proceeds in phases. The phase order is Preparation, Work, ReturningHome, and Harvest (for rounds that end in a harvest)." .


###  http://www.semanticweb.org/danielhadad/AgriGame#PlayerCollection
:PlayerCollection rdf:type owl:Class ;
                  rdfs:subClassOf :CardSet ;
                  rdfs:comment "A collection of cards from various decks curated by a player or players. May change over time." .


###  http://www.semanticweb.org/danielhadad/AgriGame#PlayerCountActionSpace
:PlayerCountActionSpace rdf:type owl:Class ;
                        rdfs:subClassOf :ActionSpace ;
                        owl:disjointWith :RoundActionSpace ;
                        rdfs:comment "The action spaces that are always available from the start of round 1, depending on the number of players in the game." .


###  http://www.semanticweb.org/danielhadad/AgriGame#PlayerToken
:PlayerToken rdf:type owl:Class ;
             rdfs:subClassOf :GameMarker ;
             rdfs:comment "The colored game pieces given to each player during game set up. These represent fixed quantities." .


###  http://www.semanticweb.org/danielhadad/AgriGame#PublishedDeck
:PublishedDeck rdf:type owl:Class ;
               rdfs:subClassOf :Deck ;
               owl:disjointWith :UnofficialDeck ;
               rdfs:comment "Individuals in this class represent decks that have been officially published." .


###  http://www.semanticweb.org/danielhadad/AgriGame#Resource
:Resource rdf:type owl:Class ;
          rdfs:subClassOf :GoodsAndFood .


###  http://www.semanticweb.org/danielhadad/AgriGame#Room
:Room rdf:type owl:Class ;
      rdfs:subClassOf :FarmyardSpace .


###  http://www.semanticweb.org/danielhadad/AgriGame#RoundActionSpace
:RoundActionSpace rdf:type owl:Class ;
                  rdfs:subClassOf :ActionSpace ;
                  rdfs:comment "The action spaces that become available as the game progresses from one round to the next." .


###  http://www.semanticweb.org/danielhadad/AgriGame#SimilarUse
:SimilarUse rdf:type owl:Class ;
            rdfs:subClassOf :Category .


###  http://www.semanticweb.org/danielhadad/AgriGame#Stage1ActionSpace
:Stage1ActionSpace rdf:type owl:Class ;
                   owl:equivalentClass [ rdf:type owl:Class ;
                                         owl:oneOf ( :FencesSpace
                                                     :MajorMinorSpace
                                                     :SowBakeSpace
                                                     <http://www.semanticweb.org/danielhadad/AgriGame#1SheepSpace>
                                                   )
                                       ] ;
                   rdfs:subClassOf :RoundActionSpace ;
                   rdfs:comment "The action spaces that become available at the start of rounds 1, 2, 3, and 4." .


###  http://www.semanticweb.org/danielhadad/AgriGame#Stage2ActionSpace
:Stage2ActionSpace rdf:type owl:Class ;
                   owl:equivalentClass [ rdf:type owl:Class ;
                                         owl:oneOf ( :FGSpace
                                                     :RenoImpSpace
                                                     <http://www.semanticweb.org/danielhadad/AgriGame#1StoneStage2Space>
                                                   )
                                       ] ;
                   rdfs:subClassOf :RoundActionSpace ;
                   rdfs:comment "The action spaces that become available at the start of rounds 5, 6, and 7." .


###  http://www.semanticweb.org/danielhadad/AgriGame#Stage3ActionSpace
:Stage3ActionSpace rdf:type owl:Class ;
                   owl:equivalentClass [ rdf:type owl:Class ;
                                         owl:oneOf ( :Take1VegSpace
                                                     <http://www.semanticweb.org/danielhadad/AgriGame#1BoarSpace>
                                                   )
                                       ] ;
                   rdfs:subClassOf :RoundActionSpace ;
                   rdfs:comment "The action spaces that become available at the start of rounds 8 and 9." .


###  http://www.semanticweb.org/danielhadad/AgriGame#Stage4ActionSpace
:Stage4ActionSpace rdf:type owl:Class ;
                   owl:equivalentClass [ rdf:type owl:Class ;
                                         owl:oneOf ( <http://www.semanticweb.org/danielhadad/AgriGame#1CowSpace>
                                                     <http://www.semanticweb.org/danielhadad/AgriGame#1StoneStage4Space>
                                                   )
                                       ] ;
                   rdfs:subClassOf :RoundActionSpace ;
                   rdfs:comment "The action spaces that become available at the start of rounds 10 and 11." .


###  http://www.semanticweb.org/danielhadad/AgriGame#Stage5ActionSpace
:Stage5ActionSpace rdf:type owl:Class ;
                   owl:equivalentClass [ rdf:type owl:Class ;
                                         owl:oneOf ( :FGWithoutRoomSpace
                                                     :PlowSowSpace
                                                   )
                                       ] ;
                   rdfs:subClassOf :RoundActionSpace ;
                   rdfs:comment "The action spaces that become available at the start of rounds 12 and 13." .


###  http://www.semanticweb.org/danielhadad/AgriGame#Stage6ActionSpace
:Stage6ActionSpace rdf:type owl:Class ;
                   owl:equivalentClass [ rdf:type owl:Class ;
                                         owl:oneOf ( :RenoFenceSpace
                                                   )
                                       ] ;
                   rdfs:subClassOf :RoundActionSpace ;
                   rdfs:comment "The action space that becomes available at the start of round 14." .


###  http://www.semanticweb.org/danielhadad/AgriGame#Strategy
:Strategy rdf:type owl:Class ;
          rdfs:subClassOf :Category .


###  http://www.semanticweb.org/danielhadad/AgriGame#UnofficialDeck
:UnofficialDeck rdf:type owl:Class ;
                rdfs:subClassOf :Deck ;
                rdfs:comment "Individuals in this class represent decks that have not been officially published but are recognized by the play-agricola community as constituting a singular deck." .


###  http://www.semanticweb.org/danielhadad/AgriGame#UweRevised
:UweRevised rdf:type owl:Class ;
            rdfs:subClassOf :Category .


###  http://www.semanticweb.org/danielhadad/AgriGame#1PlusOccupation
<http://www.semanticweb.org/danielhadad/AgriGame#1PlusOccupation> rdf:type owl:Class ;
                                                                                    rdfs:subClassOf :Occupation .


###  http://www.semanticweb.org/danielhadad/AgriGame#3PlayerActionSpace
<http://www.semanticweb.org/danielhadad/AgriGame#3PlayerActionSpace> rdf:type owl:Class ;
                                                                                       rdfs:subClassOf :PlayerCountActionSpace ;
                                                                                       rdfs:comment "The action spaces that are placed on the game board during set up for a 3 player game." .


###  http://www.semanticweb.org/danielhadad/AgriGame#3PlusOccupation
<http://www.semanticweb.org/danielhadad/AgriGame#3PlusOccupation> rdf:type owl:Class ;
                                                                                    rdfs:subClassOf :Occupation .


###  http://www.semanticweb.org/danielhadad/AgriGame#4PlayerActionSpace
<http://www.semanticweb.org/danielhadad/AgriGame#4PlayerActionSpace> rdf:type owl:Class ;
                                                                                       rdfs:subClassOf :PlayerCountActionSpace ;
                                                                                       rdfs:comment "The action spaces that are placed on the game board during set up for a 4 player game." .


###  http://www.semanticweb.org/danielhadad/AgriGame#4PlusOccupation
<http://www.semanticweb.org/danielhadad/AgriGame#4PlusOccupation> rdf:type owl:Class ;
                                                                                    rdfs:subClassOf :Occupation .


###  http://www.semanticweb.org/danielhadad/AgriGame#5PlayerActionSpace
<http://www.semanticweb.org/danielhadad/AgriGame#5PlayerActionSpace> rdf:type owl:Class ;
                                                                                       rdfs:subClassOf :PlayerCountActionSpace ;
                                                                                       rdfs:comment "The action spaces that are placed on the game board during set up for a 5 player game." .


#################################################################
#    Individuals
#################################################################

###  http://www.semanticweb.org/danielhadad/AgriGame#BaseSet
<http://www.semanticweb.org/danielhadad/AgriGameBaseSet> rdf:type owl:NamedIndividual ,
                                                                                    :PlayerCollection .


###  http://www.semanticweb.org/danielhadad/AgriGame#Cost1Imp
<http://www.semanticweb.org/danielhadad/AgriGame#Cost1Imp> rdf:type owl:NamedIndividual ,
                                                                                     :CardCost ;
                                                                            :hasValue :PlayedImp ;
                                                                            :hasAmount 1 .


###  http://www.semanticweb.org/danielhadad/AgriGame#Cost1Occ
<http://www.semanticweb.org/danielhadad/AgriGame#Cost1Occ> rdf:type owl:NamedIndividual ,
                                                                                     :CardCost ;
                                                                            :hasValue :PlayedOcc ;
                                                                            :hasAmount 1 .


###  http://www.semanticweb.org/danielhadad/AgriGame#Cost2Imp
<http://www.semanticweb.org/danielhadad/AgriGame#Cost2Imp> rdf:type owl:NamedIndividual ,
                                                                                     :CardCost ;
                                                                            :hasValue :PlayedImp ;
                                                                            :hasAmount 2 .


###  http://www.semanticweb.org/danielhadad/AgriGame#Cost2Occ
<http://www.semanticweb.org/danielhadad/AgriGame#Cost2Occ> rdf:type owl:NamedIndividual ,
                                                                                     :CardCost ;
                                                                            :hasValue :PlayedOcc ;
                                                                            :hasAmount 2 .


###  http://www.semanticweb.org/danielhadad/AgriGame#Cost3Imp
<http://www.semanticweb.org/danielhadad/AgriGame#Cost3Imp> rdf:type owl:NamedIndividual ,
                                                                                     :CardCost ;
                                                                            :hasValue :PlayedImp ;
                                                                            :hasAmount 3 .


###  http://www.semanticweb.org/danielhadad/AgriGame#Cost3Occ
<http://www.semanticweb.org/danielhadad/AgriGame#Cost3Occ> rdf:type owl:NamedIndividual ,
                                                                                     :CardCost ;
                                                                            :hasValue :PlayedOcc ;
                                                                            :hasAmount 3 .


###  http://www.semanticweb.org/danielhadad/AgriGame#Cost4Occ
<http://www.semanticweb.org/danielhadad/AgriGame#Cost4Occ> rdf:type owl:NamedIndividual ,
                                                                                     :CardCost ;
                                                                            :hasValue :PlayedOcc ;
                                                                            :hasAmount 4 .


###  http://www.semanticweb.org/danielhadad/AgriGame#Cost5Occ
<http://www.semanticweb.org/danielhadad/AgriGame#Cost5Occ> rdf:type owl:NamedIndividual ,
                                                                                     :CardCost ;
                                                                            :hasValue :PlayedOcc ;
                                                                            :hasAmount 5 .


###  http://www.semanticweb.org/danielhadad/AgriGame#Cost6Occ
<http://www.semanticweb.org/danielhadad/AgriGame#Cost6Occ> rdf:type owl:NamedIndividual ,
                                                                                     :CardCost ;
                                                                            :hasValue :PlayedOcc ;
                                                                            :hasAmount 6 .


###  http://www.semanticweb.org/danielhadad/AgriGame#Cost7Occ
<http://www.semanticweb.org/danielhadad/AgriGame#Cost7Occ> rdf:type owl:NamedIndividual ,
                                                                                     :CardCost ;
                                                                            :hasValue :PlayedOcc ;
                                                                            :hasAmount 7 .


###  http://www.semanticweb.org/danielhadad/AgriGame#CostNoOcc
<http://www.semanticweb.org/danielhadad/AgriGame#CostNoOcc> rdf:type owl:NamedIndividual ,
                                                                                      :CardCost ;
                                                                             :hasValue :PlayedOcc ;
                                                                             :hasAmount 0 .


###  http://www.semanticweb.org/danielhadad/AgriGame#Z-Man
<http://www.semanticweb.org/danielhadad/AgriGame#Z-Man> rdf:type owl:NamedIndividual ,
                                                                                  <http://www.semanticweb.org/danielhadad/AgriGamePublisher> .


###  http://www.semanticweb.org/danielhadad/AgriGame#BakeAct
:BakeAct rdf:type owl:NamedIndividual ,
                  :Action .


###  http://www.semanticweb.org/danielhadad/AgriGame#BeggingCardToken
:BeggingCardToken rdf:type owl:NamedIndividual ,
                           :GameMarker ;
                  rdfs:comment "Whenever a player cannot adequately feed their family during a harvest, or via the effects of certain cards, a player must add a Begging Card to their farm. At the end of the game, each Begging Card is worth -3 points." .


###  http://www.semanticweb.org/danielhadad/AgriGame#BigHouse
:BigHouse rdf:type owl:NamedIndividual ,
                   :Strategy ;
          rdfs:comment "A strategic approach where the player builds a house with a large number (5+) of rooms." .


###  http://www.semanticweb.org/danielhadad/AgriGame#BigImpPoints
:BigImpPoints rdf:type owl:NamedIndividual ,
                       :Strategy ;
              rdfs:comment "A strategic approach where the player aims to acquire a large number of victory points from building Improvements." .


###  http://www.semanticweb.org/danielhadad/AgriGame#BonusGrp
:BonusGrp rdf:type owl:NamedIndividual ,
                   :Designation ;
          rdfs:comment "Category of cards that have a symbol for positive or negative bonus points" .


###  http://www.semanticweb.org/danielhadad/AgriGame#BreadGrp
:BreadGrp rdf:type owl:NamedIndividual ,
                   :Designation ;
          rdfs:comment "Category of cards that have the Bake Bread symbol" .


###  http://www.semanticweb.org/danielhadad/AgriGame#BuildFencesAct
:BuildFencesAct rdf:type owl:NamedIndividual ,
                         :Action .


###  http://www.semanticweb.org/danielhadad/AgriGame#BuildRoomAct
:BuildRoomAct rdf:type owl:NamedIndividual ,
                       :Action .


###  http://www.semanticweb.org/danielhadad/AgriGame#BuildSpace
:BuildSpace rdf:type owl:NamedIndividual ,
                     :BoardActionSpace ;
            rdfs:label "Build Room(s) and/or Stable(s)" .


###  http://www.semanticweb.org/danielhadad/AgriGame#BuildStableAct
:BuildStableAct rdf:type owl:NamedIndividual ,
                         :Action .


###  http://www.semanticweb.org/danielhadad/AgriGame#CHGrp
:CHGrp rdf:type owl:NamedIndividual ,
                :Designation .


###  http://www.semanticweb.org/danielhadad/AgriGame#Cattle
:Cattle rdf:type owl:NamedIndividual ,
                 :Animal .


###  http://www.semanticweb.org/danielhadad/AgriGame#CheapOccSpace
:CheapOccSpace rdf:type owl:NamedIndividual ,
                        :BoardActionSpace ;
               rdfs:comment "A player's first occupation is free, each additional one costs 1 Food" ;
               rdfs:label "1 Occupation" .


###  http://www.semanticweb.org/danielhadad/AgriGame#Clay
:Clay rdf:type owl:NamedIndividual ,
               :BuildingResource .


###  http://www.semanticweb.org/danielhadad/AgriGame#ClayHutRoom
:ClayHutRoom rdf:type owl:NamedIndividual ,
                      :Room .


###  http://www.semanticweb.org/danielhadad/AgriGame#CookGrp
:CookGrp rdf:type owl:NamedIndividual ,
                  :Designation ;
         rdfs:comment "Category of improvments with the cooking symbol." .


###  http://www.semanticweb.org/danielhadad/AgriGame#Cost1Bo
:Cost1Bo rdf:type owl:NamedIndividual ,
                  :CardCost ;
         :hasValue :WildBoar ;
         :hasAmount 1 .


###  http://www.semanticweb.org/danielhadad/AgriGame#Cost1C
:Cost1C rdf:type owl:NamedIndividual ,
                 :CardCost ;
        :hasValue :Clay ;
        :hasAmount 1 .


###  http://www.semanticweb.org/danielhadad/AgriGame#Cost1Ca
:Cost1Ca rdf:type owl:NamedIndividual ,
                  :CardCost ;
         :hasValue :Cattle ;
         :hasAmount 1 .


###  http://www.semanticweb.org/danielhadad/AgriGame#Cost1F
:Cost1F rdf:type owl:NamedIndividual ,
                 :CardCost ;
        :hasValue :Food ;
        :hasAmount 1 .


###  http://www.semanticweb.org/danielhadad/AgriGame#Cost1G
:Cost1G rdf:type owl:NamedIndividual ,
                 :CardCost ;
        :hasValue :Grain ;
        :hasAmount 1 .


###  http://www.semanticweb.org/danielhadad/AgriGame#Cost1R
:Cost1R rdf:type owl:NamedIndividual ,
                 :CardCost ;
        :hasValue :Reed ;
        :hasAmount 1 .


###  http://www.semanticweb.org/danielhadad/AgriGame#Cost1S
:Cost1S rdf:type owl:NamedIndividual ,
                 :CardCost ;
        :hasValue :Stone ;
        :hasAmount 1 .


###  http://www.semanticweb.org/danielhadad/AgriGame#Cost1Sh
:Cost1Sh rdf:type owl:NamedIndividual ,
                  :CardCost ;
         :hasValue :Sheep ;
         :hasAmount 1 .


###  http://www.semanticweb.org/danielhadad/AgriGame#Cost1V
:Cost1V rdf:type owl:NamedIndividual ,
                 :CardCost ;
        :hasValue :Vegetable ;
        :hasAmount 1 .


###  http://www.semanticweb.org/danielhadad/AgriGame#Cost1W
:Cost1W rdf:type owl:NamedIndividual ,
                 :CardCost ;
        :hasValue :Wood ;
        :hasAmount 1 .


###  http://www.semanticweb.org/danielhadad/AgriGame#Cost2Bo
:Cost2Bo rdf:type owl:NamedIndividual ,
                  :CardCost ;
         :hasValue :WildBoar ;
         :hasAmount 2 .


###  http://www.semanticweb.org/danielhadad/AgriGame#Cost2C
:Cost2C rdf:type owl:NamedIndividual ,
                 :CardCost ;
        :hasValue :Clay ;
        :hasAmount 2 .


###  http://www.semanticweb.org/danielhadad/AgriGame#Cost2Ca
:Cost2Ca rdf:type owl:NamedIndividual ,
                  :CardCost ;
         :hasValue :Cattle ;
         :hasAmount 2 .


###  http://www.semanticweb.org/danielhadad/AgriGame#Cost2F
:Cost2F rdf:type owl:NamedIndividual ,
                 :CardCost ;
        :hasValue :Food ;
        :hasAmount 2 .


###  http://www.semanticweb.org/danielhadad/AgriGame#Cost2G
:Cost2G rdf:type owl:NamedIndividual ,
                 :CardCost ;
        :hasValue :Grain ;
        :hasAmount 2 .


###  http://www.semanticweb.org/danielhadad/AgriGame#Cost2R
:Cost2R rdf:type owl:NamedIndividual ,
                 :CardCost ;
        :hasValue :Reed ;
        :hasAmount 2 .


###  http://www.semanticweb.org/danielhadad/AgriGame#Cost2S
:Cost2S rdf:type owl:NamedIndividual ,
                 :CardCost ;
        :hasValue :Stone ;
        :hasAmount 2 .


###  http://www.semanticweb.org/danielhadad/AgriGame#Cost2Sh
:Cost2Sh rdf:type owl:NamedIndividual ,
                  :CardCost ;
         :hasValue :Sheep ;
         :hasAmount 2 .


###  http://www.semanticweb.org/danielhadad/AgriGame#Cost2V
:Cost2V rdf:type owl:NamedIndividual ,
                 :CardCost ;
        :hasValue :Vegetable ;
        :hasAmount 2 .


###  http://www.semanticweb.org/danielhadad/AgriGame#Cost2W
:Cost2W rdf:type owl:NamedIndividual ,
                 :CardCost ;
        :hasValue :Wood ;
        :hasAmount 2 .


###  http://www.semanticweb.org/danielhadad/AgriGame#Cost3Bo
:Cost3Bo rdf:type owl:NamedIndividual ,
                  :CardCost ;
         :hasValue :WildBoar ;
         :hasAmount 3 .


###  http://www.semanticweb.org/danielhadad/AgriGame#Cost3C
:Cost3C rdf:type owl:NamedIndividual ,
                 :CardCost ;
        :hasValue :Clay ;
        :hasAmount 3 .


###  http://www.semanticweb.org/danielhadad/AgriGame#Cost3Ca
:Cost3Ca rdf:type owl:NamedIndividual ,
                  :CardCost ;
         :hasValue :Cattle ;
         :hasAmount 3 .


###  http://www.semanticweb.org/danielhadad/AgriGame#Cost3F
:Cost3F rdf:type owl:NamedIndividual ,
                 :CardCost ;
        :hasValue :Food ;
        :hasAmount 3 .


###  http://www.semanticweb.org/danielhadad/AgriGame#Cost3G
:Cost3G rdf:type owl:NamedIndividual ,
                 :CardCost ;
        :hasValue :Grain ;
        :hasAmount 3 .


###  http://www.semanticweb.org/danielhadad/AgriGame#Cost3R
:Cost3R rdf:type owl:NamedIndividual ,
                 :CardCost ;
        :hasValue :Reed ;
        :hasAmount 3 .


###  http://www.semanticweb.org/danielhadad/AgriGame#Cost3S
:Cost3S rdf:type owl:NamedIndividual ,
                 :CardCost ;
        :hasValue :Stone ;
        :hasAmount 3 .


###  http://www.semanticweb.org/danielhadad/AgriGame#Cost3Sh
:Cost3Sh rdf:type owl:NamedIndividual ,
                  :CardCost ;
         :hasValue :Sheep ;
         :hasAmount 3 .


###  http://www.semanticweb.org/danielhadad/AgriGame#Cost3V
:Cost3V rdf:type owl:NamedIndividual ,
                 :CardCost ;
        :hasValue :Vegetable ;
        :hasAmount 3 .


###  http://www.semanticweb.org/danielhadad/AgriGame#Cost3W
:Cost3W rdf:type owl:NamedIndividual ,
                 :CardCost ;
        :hasValue :Wood ;
        :hasAmount 3 .


###  http://www.semanticweb.org/danielhadad/AgriGame#Cost4Bo
:Cost4Bo rdf:type owl:NamedIndividual ,
                  :CardCost ;
         :hasValue :WildBoar ;
         :hasAmount 4 .


###  http://www.semanticweb.org/danielhadad/AgriGame#Cost4C
:Cost4C rdf:type owl:NamedIndividual ,
                 :CardCost ;
        :hasValue :Clay ;
        :hasAmount 4 .


###  http://www.semanticweb.org/danielhadad/AgriGame#Cost4Ca
:Cost4Ca rdf:type owl:NamedIndividual ,
                  :CardCost ;
         :hasValue :Cattle ;
         :hasAmount 4 .


###  http://www.semanticweb.org/danielhadad/AgriGame#Cost4F
:Cost4F rdf:type owl:NamedIndividual ,
                 :CardCost ;
        :hasValue :Food ;
        :hasAmount 4 .


###  http://www.semanticweb.org/danielhadad/AgriGame#Cost4G
:Cost4G rdf:type owl:NamedIndividual ,
                 :CardCost ;
        :hasValue :Grain ;
        :hasAmount 4 .


###  http://www.semanticweb.org/danielhadad/AgriGame#Cost4R
:Cost4R rdf:type owl:NamedIndividual ,
                 :CardCost ;
        :hasValue :Reed ;
        :hasAmount 4 .


###  http://www.semanticweb.org/danielhadad/AgriGame#Cost4S
:Cost4S rdf:type owl:NamedIndividual ,
                 :CardCost ;
        :hasValue :Stone ;
        :hasAmount 4 .


###  http://www.semanticweb.org/danielhadad/AgriGame#Cost4Sh
:Cost4Sh rdf:type owl:NamedIndividual ,
                  :CardCost ;
         :hasValue :Sheep ;
         :hasAmount 4 .


###  http://www.semanticweb.org/danielhadad/AgriGame#Cost4V
:Cost4V rdf:type owl:NamedIndividual ,
                 :CardCost ;
        :hasValue :Vegetable ;
        :hasAmount 4 .


###  http://www.semanticweb.org/danielhadad/AgriGame#Cost4W
:Cost4W rdf:type owl:NamedIndividual ,
                 :CardCost ;
        :hasValue :Wood ;
        :hasAmount 4 .


###  http://www.semanticweb.org/danielhadad/AgriGame#Cost5Bo
:Cost5Bo rdf:type owl:NamedIndividual ,
                  :CardCost ;
         :hasValue :WildBoar ;
         :hasAmount 5 .


###  http://www.semanticweb.org/danielhadad/AgriGame#Cost5C
:Cost5C rdf:type owl:NamedIndividual ,
                 :CardCost ;
        :hasValue :Clay ;
        :hasAmount 5 .


###  http://www.semanticweb.org/danielhadad/AgriGame#Cost5Ca
:Cost5Ca rdf:type owl:NamedIndividual ,
                  :CardCost ;
         :hasValue :Cattle ;
         :hasAmount 5 .


###  http://www.semanticweb.org/danielhadad/AgriGame#Cost5F
:Cost5F rdf:type owl:NamedIndividual ,
                 :CardCost ;
        :hasValue :Food ;
        :hasAmount 5 .


###  http://www.semanticweb.org/danielhadad/AgriGame#Cost5G
:Cost5G rdf:type owl:NamedIndividual ,
                 :CardCost ;
        :hasValue :Grain ;
        :hasAmount 5 .


###  http://www.semanticweb.org/danielhadad/AgriGame#Cost5R
:Cost5R rdf:type owl:NamedIndividual ,
                 :CardCost ;
        :hasValue :Reed ;
        :hasAmount 5 .


###  http://www.semanticweb.org/danielhadad/AgriGame#Cost5S
:Cost5S rdf:type owl:NamedIndividual ,
                 :CardCost ;
        :hasValue :Stone ;
        :hasAmount 5 .


###  http://www.semanticweb.org/danielhadad/AgriGame#Cost5Sh
:Cost5Sh rdf:type owl:NamedIndividual ,
                  :CardCost ;
         :hasValue :Sheep ;
         :hasAmount 5 .


###  http://www.semanticweb.org/danielhadad/AgriGame#Cost5V
:Cost5V rdf:type owl:NamedIndividual ,
                 :CardCost ;
        :hasValue :Vegetable ;
        :hasAmount 5 .


###  http://www.semanticweb.org/danielhadad/AgriGame#Cost5W
:Cost5W rdf:type owl:NamedIndividual ,
                 :CardCost ;
        :hasValue :Wood ;
        :hasAmount 5 .


###  http://www.semanticweb.org/danielhadad/AgriGame#DLCombo
:DLCombo rdf:type owl:NamedIndividual ,
                  :SimilarUse ;
         rdfs:comment "The category of cards that add effects to the Day Laborer action space." .


###  http://www.semanticweb.org/danielhadad/AgriGame#DLSpace
:DLSpace rdf:type owl:NamedIndividual ,
                  :BoardActionSpace ;
         rdfs:label "Day Laborer" .


###  http://www.semanticweb.org/danielhadad/AgriGame#E
:E rdf:type owl:NamedIndividual ,
            :PublishedDeck ;
   rdfs:label "E Deck" .


###  http://www.semanticweb.org/danielhadad/AgriGame#EarlyClayRen
:EarlyClayRen rdf:type owl:NamedIndividual ,
                       :Strategy ;
              rdfs:comment "A strategic approach where the player renovated to Clay early to leverage the effect of particular cards." .


###  http://www.semanticweb.org/danielhadad/AgriGame#EarlyCrops
:EarlyCrops rdf:type owl:NamedIndividual ,
                     :Strategy ;
            rdfs:comment "A strategic approach where the player plows fields and sows grain and/or vegetables in the early Stages of the game." .


###  http://www.semanticweb.org/danielhadad/AgriGame#EarlyStoneRen
:EarlyStoneRen rdf:type owl:NamedIndividual ,
                        :Strategy ;
               rdfs:comment "A strategic approach where the player renovates to Stone early to leverage the effects of particular cards." .


###  http://www.semanticweb.org/danielhadad/AgriGame#EmptyField
:EmptyField rdf:type owl:NamedIndividual ,
                     :Field .


###  http://www.semanticweb.org/danielhadad/AgriGame#ExpensiveOccSpace
:ExpensiveOccSpace rdf:type owl:NamedIndividual ,
                            <http://www.semanticweb.org/danielhadad/AgriGame#4PlayerActionSpace> ;
                   rdfs:comment "A player's first and second Occupation cost 1 Food each. Each Occupation after that costs 2 Food." ;
                   rdfs:label "1 Occupation" .


###  http://www.semanticweb.org/danielhadad/AgriGame#FGAct
:FGAct rdf:type owl:NamedIndividual ,
                :Action .


###  http://www.semanticweb.org/danielhadad/AgriGame#FGSpace
:FGSpace rdf:type owl:NamedIndividual ,
                  :Stage2ActionSpace ;
         rdfs:label "After Family Growth also 1 Minor Improvement" .


###  http://www.semanticweb.org/danielhadad/AgriGame#FGWithoutRoomAct
:FGWithoutRoomAct rdf:type owl:NamedIndividual ,
                           :Action .


###  http://www.semanticweb.org/danielhadad/AgriGame#FGWithoutRoomSpace
:FGWithoutRoomSpace rdf:type owl:NamedIndividual ,
                             :Stage5ActionSpace ;
                    rdfs:label "Family Growth even without space in your home" .


###  http://www.semanticweb.org/danielhadad/AgriGame#FPGrp
:FPGrp rdf:type owl:NamedIndividual ,
                :Designation .


###  http://www.semanticweb.org/danielhadad/AgriGame#FeedingEngine
:FeedingEngine rdf:type owl:NamedIndividual ,
                        :SimilarUse ;
               rdfs:comment "The category of cards that are an important part of creating sustainable feeding for the player." .


###  http://www.semanticweb.org/danielhadad/AgriGame#Fence
:Fence rdf:type owl:NamedIndividual ,
                :PlayerToken .


###  http://www.semanticweb.org/danielhadad/AgriGame#FencedStable
:FencedStable rdf:type owl:NamedIndividual ,
                       :FarmyardSpace .


###  http://www.semanticweb.org/danielhadad/AgriGame#FencesSpace
:FencesSpace rdf:type owl:NamedIndividual ,
                      :Stage1ActionSpace ;
             rdfs:label "Fences" .


###  http://www.semanticweb.org/danielhadad/AgriGame#FishCombo
:FishCombo rdf:type owl:NamedIndividual ,
                    :SimilarUse ;
           rdfs:comment "The category of cards that add effects to the Fishing action space." .


###  http://www.semanticweb.org/danielhadad/AgriGame#FishingSpace
:FishingSpace rdf:type owl:NamedIndividual ,
                       :BoardActionSpace ;
              rdfs:label "Fishing" .


###  http://www.semanticweb.org/danielhadad/AgriGame#Food
:Food rdf:type owl:NamedIndividual ,
               :GoodsAndFood .


###  http://www.semanticweb.org/danielhadad/AgriGame#Fr
:Fr rdf:type owl:NamedIndividual ,
             :PublishedDeck ;
    rdfs:label "France Deck" .


###  http://www.semanticweb.org/danielhadad/AgriGame#G
:G rdf:type owl:NamedIndividual ,
            :PublishedDeck ;
   rdfs:label "Gamer Deck" .


###  http://www.semanticweb.org/danielhadad/AgriGame#G4
:G4 rdf:type owl:NamedIndividual ,
             :UnofficialDeck .


###  http://www.semanticweb.org/danielhadad/AgriGame#G5
:G5 rdf:type owl:NamedIndividual ,
             :UnofficialDeck .


###  http://www.semanticweb.org/danielhadad/AgriGame#G6
:G6 rdf:type owl:NamedIndividual ,
             :UnofficialDeck .


###  http://www.semanticweb.org/danielhadad/AgriGame#G7
:G7 rdf:type owl:NamedIndividual ,
             :UnofficialDeck .


###  http://www.semanticweb.org/danielhadad/AgriGame#GetBreedingPair
:GetBreedingPair rdf:type owl:NamedIndividual ,
                          :Strategy ;
                 rdfs:comment "A strategic approach where the player gains the ability to hold at least 3 animals of the same kind" .


###  http://www.semanticweb.org/danielhadad/AgriGame#Grain
:Grain rdf:type owl:NamedIndividual ,
                :Crop .


###  http://www.semanticweb.org/danielhadad/AgriGame#GuestToken
:GuestToken rdf:type owl:NamedIndividual ,
                     :GameMarker ;
            rdfs:comment "A token representing a temporary person on a player's farm or the board." .


###  http://www.semanticweb.org/danielhadad/AgriGame#GuildGrp
:GuildGrp rdf:type owl:NamedIndividual ,
                   :Designation ;
          rdfs:comment "The category including the Joinery, Pottery, Basket Maker's Workshop, and their respective upgrades." .


###  http://www.semanticweb.org/danielhadad/AgriGame#HarvestBreedingPhase
:HarvestBreedingPhase rdf:type owl:NamedIndividual ,
                               :HarvestPhase ;
                      rdfs:comment "If a player has at least two animals of the same type, the animals breed to process a newborn animal. The newborn animal must be housed on the player's farm and cannot be converted to food during this phase." .


###  http://www.semanticweb.org/danielhadad/AgriGame#HarvestFeedingPhase
:HarvestFeedingPhase rdf:type owl:NamedIndividual ,
                              :HarvestPhase ;
                     rdfs:comment "In this phase, players must pay an appropriate amount of Food in order to feed their families." .


###  http://www.semanticweb.org/danielhadad/AgriGame#HarvestFieldPhase
:HarvestFieldPhase rdf:type owl:NamedIndividual ,
                            :HarvestPhase ;
                   rdfs:comment "The first phase of a harvest. Many card effects resolve during this phase. Fields are harvested." .


###  http://www.semanticweb.org/danielhadad/AgriGame#HarvestFood
:HarvestFood rdf:type owl:NamedIndividual ,
                      :SimilarUse ;
             rdfs:comment "The category of cards that provide food during the Harvest, either passively through met farm conditions, or by allowing the conversion of Goods to Food during the Harvest specifically." .


###  http://www.semanticweb.org/danielhadad/AgriGame#I
:I rdf:type owl:NamedIndividual ,
            :PublishedDeck ;
   rdfs:label "I Deck" .


###  http://www.semanticweb.org/danielhadad/AgriGame#K
:K rdf:type owl:NamedIndividual ,
            :PublishedDeck ;
   rdfs:label "K Deck" .


###  http://www.semanticweb.org/danielhadad/AgriGame#MajorMinorSpace
:MajorMinorSpace rdf:type owl:NamedIndividual ,
                          :Stage1ActionSpace ;
                 rdfs:label "1 Major or Minor Improvement" .


###  http://www.semanticweb.org/danielhadad/AgriGame#MakeUnblockable
:MakeUnblockable rdf:type owl:NamedIndividual ,
                          :SimilarUse ;
                 rdfs:comment "Cards in this category allow players to use specific action spaces even if they are occupied by an opponent" .


###  http://www.semanticweb.org/danielhadad/AgriGame#MinorPlowGrp
:MinorPlowGrp rdf:type owl:NamedIndividual ,
                       :Designation ;
              rdfs:comment "The category of cards that count as minor Plows" .


###  http://www.semanticweb.org/danielhadad/AgriGame#NextFGWithout
:NextFGWithout rdf:type owl:NamedIndividual ,
                        :SimilarUse ;
               rdfs:comment "The category of cards that allow the player to use the Stage 2 FG action space even without room in their home." .


###  http://www.semanticweb.org/danielhadad/AgriGame#NurFG
:NurFG rdf:type owl:NamedIndividual ,
                :Strategy ;
       rdfs:comment "A strategic approach in which the player aims to acquire resources to build one or more additional rooms and grow their family as soon as possible." .


###  http://www.semanticweb.org/danielhadad/AgriGame#OccOrFGSpace
:OccOrFGSpace rdf:type owl:NamedIndividual ,
                       <http://www.semanticweb.org/danielhadad/AgriGame#5PlayerActionSpace> ;
              rdfs:comment "A player's first and second Occupations cost 1 Food each. Each additional Occupation costs 2 Food" ;
              rdfs:label "1 Occupation or, From Round 5, Family Growth" .


###  http://www.semanticweb.org/danielhadad/AgriGame#OnceInClay
:OnceInClay rdf:type owl:NamedIndividual ,
                     :SimilarUse ;
            rdfs:comment "The category of cards that have no effect unless the player lives in (at least) a Clay Hut." ,
                         "The category of cards that have no effect unless the player lives in a Stone House." .


###  http://www.semanticweb.org/danielhadad/AgriGame#OnceInStone
:OnceInStone rdf:type owl:NamedIndividual ,
                      :SimilarUse .


###  http://www.semanticweb.org/danielhadad/AgriGame#OriginalVersion
:OriginalVersion rdf:type owl:NamedIndividual ,
                          :GameVersion .


###  http://www.semanticweb.org/danielhadad/AgriGame#OvenGrp
:OvenGrp rdf:type owl:NamedIndividual ,
                  :Designation ;
         rdfs:comment "Category of improvements that count as Ovens" .


###  http://www.semanticweb.org/danielhadad/AgriGame#PassingMinor
:PassingMinor rdf:type owl:NamedIndividual ,
                       :Designation ;
              rdfs:comment "The category of minor improvements that must be passed to another player after being played." .


###  http://www.semanticweb.org/danielhadad/AgriGame#Pasture
:Pasture rdf:type owl:NamedIndividual ,
                  :FarmyardSpace .


###  http://www.semanticweb.org/danielhadad/AgriGame#Person
:Person rdf:type owl:NamedIndividual ,
                 :PlayerToken .


###  http://www.semanticweb.org/danielhadad/AgriGame#PlantedField
:PlantedField rdf:type owl:NamedIndividual ,
                       :Field .


###  http://www.semanticweb.org/danielhadad/AgriGame#PlayByStage1
:PlayByStage1 rdf:type owl:NamedIndividual ,
                       :SimilarUse ;
              rdfs:comment "A small category of cards that must be played before the end of Stage 1. There are other cards with timing requirements, but it is worth noting this special subset." .


###  http://www.semanticweb.org/danielhadad/AgriGame#PlayMajorMinorAct
:PlayMajorMinorAct rdf:type owl:NamedIndividual ,
                            :Action .


###  http://www.semanticweb.org/danielhadad/AgriGame#PlayMinorAct
:PlayMinorAct rdf:type owl:NamedIndividual ,
                       :Action .


###  http://www.semanticweb.org/danielhadad/AgriGame#PlayOccAct
:PlayOccAct rdf:type owl:NamedIndividual ,
                     :Action .


###  http://www.semanticweb.org/danielhadad/AgriGame#PlayedImp
:PlayedImp rdf:type owl:NamedIndividual ,
                    :FarmyardSpace .


###  http://www.semanticweb.org/danielhadad/AgriGame#PlayedOcc
:PlayedOcc rdf:type owl:NamedIndividual ,
                    :FarmyardSpace .


###  http://www.semanticweb.org/danielhadad/AgriGame#PlowAct
:PlowAct rdf:type owl:NamedIndividual ,
                  :Action .


###  http://www.semanticweb.org/danielhadad/AgriGame#PlowCombo
:PlowCombo rdf:type owl:NamedIndividual ,
                    :SimilarUse ;
           rdfs:comment "The category of cards that affect the Plow 1 Field space" .


###  http://www.semanticweb.org/danielhadad/AgriGame#PlowSowSpace
:PlowSowSpace rdf:type owl:NamedIndividual ,
                       :Stage5ActionSpace ;
              rdfs:label "Plow 1 Field and/or Sow" .


###  http://www.semanticweb.org/danielhadad/AgriGame#PlowSpace
:PlowSpace rdf:type owl:NamedIndividual ,
                    :BoardActionSpace ;
           rdfs:label "Plow 1 Field" .


###  http://www.semanticweb.org/danielhadad/AgriGame#PointCeiling
:PointCeiling rdf:type owl:NamedIndividual ,
                       :SimilarUse ;
              rdfs:comment "Cards in this category are used primarily to award victory points to the player directly without aiding in farm development." .


###  http://www.semanticweb.org/danielhadad/AgriGame#PondGrp
:PondGrp rdf:type owl:NamedIndividual ,
                  :SimilarUse ;
         rdfs:comment "The category of mostly point-granting minors with no play cost that add food and/or resources to future round spaces." .


###  http://www.semanticweb.org/danielhadad/AgriGame#PreparationPhase
:PreparationPhase rdf:type owl:NamedIndividual ,
                           :Phase ;
                  rdfs:comment "The first phase of a round. The new round card is flipped face up and the appropriate items are added to the board." .


###  http://www.semanticweb.org/danielhadad/AgriGame#QueueJumper
:QueueJumper rdf:type owl:NamedIndividual ,
                      :SimilarUse ;
             rdfs:comment "Cards in this category aid the player in using the FG action space \"out of turn\"." .


###  http://www.semanticweb.org/danielhadad/AgriGame#RSFSpace
:RSFSpace rdf:type owl:NamedIndividual ,
                   <http://www.semanticweb.org/danielhadad/AgriGame#4PlayerActionSpace> ;
          rdfs:comment "Take 1 Reed, 1 Stone, and 1 Food" .


###  http://www.semanticweb.org/danielhadad/AgriGame#ReceiveAnimalEffect
:ReceiveAnimalEffect rdf:type owl:NamedIndividual ,
                              :Effect .


###  http://www.semanticweb.org/danielhadad/AgriGame#ReceiveBREffect
:ReceiveBREffect rdf:type owl:NamedIndividual ,
                          :Effect .


###  http://www.semanticweb.org/danielhadad/AgriGame#ReceiveBoarEffect
:ReceiveBoarEffect rdf:type owl:NamedIndividual ,
                            :Effect .


###  http://www.semanticweb.org/danielhadad/AgriGame#ReceiveClayEffect
:ReceiveClayEffect rdf:type owl:NamedIndividual ,
                            :Effect .


###  http://www.semanticweb.org/danielhadad/AgriGame#ReceiveCowEffect
:ReceiveCowEffect rdf:type owl:NamedIndividual ,
                           :Effect .


###  http://www.semanticweb.org/danielhadad/AgriGame#ReceiveEffect
:ReceiveEffect rdf:type owl:NamedIndividual ,
                        :Effect .


###  http://www.semanticweb.org/danielhadad/AgriGame#ReceiveFenceEffect
:ReceiveFenceEffect rdf:type owl:NamedIndividual ,
                             :Effect .


###  http://www.semanticweb.org/danielhadad/AgriGame#ReceiveFieldEffect
:ReceiveFieldEffect rdf:type owl:NamedIndividual ,
                             :Effect .


###  http://www.semanticweb.org/danielhadad/AgriGame#ReceiveFoodEffect
:ReceiveFoodEffect rdf:type owl:NamedIndividual ,
                            :Effect .


###  http://www.semanticweb.org/danielhadad/AgriGame#ReceiveGoodEffect
:ReceiveGoodEffect rdf:type owl:NamedIndividual ,
                            :Effect .


###  http://www.semanticweb.org/danielhadad/AgriGame#ReceiveGrainEffect
:ReceiveGrainEffect rdf:type owl:NamedIndividual ,
                             :Effect .


###  http://www.semanticweb.org/danielhadad/AgriGame#ReceiveReedEffect
:ReceiveReedEffect rdf:type owl:NamedIndividual ,
                            :Effect .


###  http://www.semanticweb.org/danielhadad/AgriGame#ReceiveRenoEffect
:ReceiveRenoEffect rdf:type owl:NamedIndividual ,
                            :Effect .


###  http://www.semanticweb.org/danielhadad/AgriGame#ReceiveResourceEffect
:ReceiveResourceEffect rdf:type owl:NamedIndividual ,
                                :Effect .


###  http://www.semanticweb.org/danielhadad/AgriGame#ReceiveRoomEffect
:ReceiveRoomEffect rdf:type owl:NamedIndividual ,
                            :Effect .


###  http://www.semanticweb.org/danielhadad/AgriGame#ReceiveSheepEffect
:ReceiveSheepEffect rdf:type owl:NamedIndividual ,
                             :Effect .


###  http://www.semanticweb.org/danielhadad/AgriGame#ReceiveStableEffect
:ReceiveStableEffect rdf:type owl:NamedIndividual ,
                              :Effect .


###  http://www.semanticweb.org/danielhadad/AgriGame#ReceiveStoneEffect
:ReceiveStoneEffect rdf:type owl:NamedIndividual ,
                             :Effect .


###  http://www.semanticweb.org/danielhadad/AgriGame#ReceiveVegEffect
:ReceiveVegEffect rdf:type owl:NamedIndividual ,
                           :Effect .


###  http://www.semanticweb.org/danielhadad/AgriGame#ReceiveWoodEffect
:ReceiveWoodEffect rdf:type owl:NamedIndividual ,
                            :Effect .


###  http://www.semanticweb.org/danielhadad/AgriGame#Reed
:Reed rdf:type owl:NamedIndividual ,
               :BuildingResource .


###  http://www.semanticweb.org/danielhadad/AgriGame#RenoAct
:RenoAct rdf:type owl:NamedIndividual ,
                  :Action .


###  http://www.semanticweb.org/danielhadad/AgriGame#RenoDiscounter
:RenoDiscounter rdf:type owl:NamedIndividual ,
                         :SimilarUse ;
                rdfs:comment "Cards in this category lower the cost of renovation." .


###  http://www.semanticweb.org/danielhadad/AgriGame#RenoFenceSpace
:RenoFenceSpace rdf:type owl:NamedIndividual ,
                         :Stage6ActionSpace ;
                rdfs:label "After Renovation also Fences" .


###  http://www.semanticweb.org/danielhadad/AgriGame#RenoImpSpace
:RenoImpSpace rdf:type owl:NamedIndividual ,
                       :Stage2ActionSpace ;
              rdfs:label "After Renovation also 1 Major or Minor Improvement" .


###  http://www.semanticweb.org/danielhadad/AgriGame#ReturningHomePhase
:ReturningHomePhase rdf:type owl:NamedIndividual ,
                             :Phase ;
                    rdfs:comment "The clean-up phase before the end of the round (in rounds without a harvest) or the start of a harvest. Many card effects resolve during this phase. All players return their person tokens to their farms." .


###  http://www.semanticweb.org/danielhadad/AgriGame#RevisedVersion
:RevisedVersion rdf:type owl:NamedIndividual ,
                         :GameVersion .


###  http://www.semanticweb.org/danielhadad/AgriGame#RoomDiscounter
:RoomDiscounter rdf:type owl:NamedIndividual ,
                         :SimilarUse ;
                rdfs:comment "Cards in this category provide discounts to the cost of building new rooms." .


###  http://www.semanticweb.org/danielhadad/AgriGame#SPAct
:SPAct rdf:type owl:NamedIndividual ,
                :Action .


###  http://www.semanticweb.org/danielhadad/AgriGame#SPSpace
:SPSpace rdf:type owl:NamedIndividual ,
                  :BoardActionSpace ;
         rdfs:label "Starting Player and/or Minor Improvement" .


###  http://www.semanticweb.org/danielhadad/AgriGame#SPToken
:SPToken rdf:type owl:NamedIndividual ,
                  :GameMarker .


###  http://www.semanticweb.org/danielhadad/AgriGame#Sheep
:Sheep rdf:type owl:NamedIndividual ,
                :Animal .


###  http://www.semanticweb.org/danielhadad/AgriGame#SowAct
:SowAct rdf:type owl:NamedIndividual ,
                 :Action .


###  http://www.semanticweb.org/danielhadad/AgriGame#SowBakeSpace
:SowBakeSpace rdf:type owl:NamedIndividual ,
                       :Stage1ActionSpace ;
              rdfs:label "Sow and/or Bake Bread" .


###  http://www.semanticweb.org/danielhadad/AgriGame#SownGField
:SownGField rdf:type owl:NamedIndividual ,
                     :Field .


###  http://www.semanticweb.org/danielhadad/AgriGame#SownVField
:SownVField rdf:type owl:NamedIndividual ,
                     :Field .


###  http://www.semanticweb.org/danielhadad/AgriGame#Stable
:Stable rdf:type owl:NamedIndividual ,
                 :PlayerToken .


###  http://www.semanticweb.org/danielhadad/AgriGame#Stone
:Stone rdf:type owl:NamedIndividual ,
                :BuildingResource .


###  http://www.semanticweb.org/danielhadad/AgriGame#StoneHouseRoom
:StoneHouseRoom rdf:type owl:NamedIndividual ,
                         :Room .


###  http://www.semanticweb.org/danielhadad/AgriGame#TPCombo
:TPCombo rdf:type owl:NamedIndividual ,
                  :SimilarUse ;
         rdfs:comment "The category of cards that add effects to the Traveling Players action space." .


###  http://www.semanticweb.org/danielhadad/AgriGame#TPSpace
:TPSpace rdf:type owl:NamedIndividual ,
                  <http://www.semanticweb.org/danielhadad/AgriGame#4PlayerActionSpace> ;
         rdfs:comment "Traveling Players" .


###  http://www.semanticweb.org/danielhadad/AgriGame#Take1VegSpace
:Take1VegSpace rdf:type owl:NamedIndividual ,
                        :Stage3ActionSpace ;
               rdfs:label "Take 1 Vegetable" .


###  http://www.semanticweb.org/danielhadad/AgriGame#TakeAct
:TakeAct rdf:type owl:NamedIndividual ,
                  :Action .


###  http://www.semanticweb.org/danielhadad/AgriGame#TakeAnimalAct
:TakeAnimalAct rdf:type owl:NamedIndividual ,
                        :Action .


###  http://www.semanticweb.org/danielhadad/AgriGame#TakeBRAct
:TakeBRAct rdf:type owl:NamedIndividual ,
                    :Action .


###  http://www.semanticweb.org/danielhadad/AgriGame#TakeBoar
:TakeBoar rdf:type owl:NamedIndividual ,
                   :Action .


###  http://www.semanticweb.org/danielhadad/AgriGame#TakeClayAct
:TakeClayAct rdf:type owl:NamedIndividual ,
                      :Action .


###  http://www.semanticweb.org/danielhadad/AgriGame#TakeCowAct
:TakeCowAct rdf:type owl:NamedIndividual ,
                     :Action .


###  http://www.semanticweb.org/danielhadad/AgriGame#TakeFoodAct
:TakeFoodAct rdf:type owl:NamedIndividual ,
                      :Action .


###  http://www.semanticweb.org/danielhadad/AgriGame#TakeGoodAct
:TakeGoodAct rdf:type owl:NamedIndividual .


###  http://www.semanticweb.org/danielhadad/AgriGame#TakeGrainAct
:TakeGrainAct rdf:type owl:NamedIndividual ,
                       :Action .


###  http://www.semanticweb.org/danielhadad/AgriGame#TakeGrainSpace
:TakeGrainSpace rdf:type owl:NamedIndividual ,
                         :BoardActionSpace ;
                rdfs:label "Take 1 Grain" .


###  http://www.semanticweb.org/danielhadad/AgriGame#TakeReedAct
:TakeReedAct rdf:type owl:NamedIndividual ,
                      :Action .


###  http://www.semanticweb.org/danielhadad/AgriGame#TakeResourceAct
:TakeResourceAct rdf:type owl:NamedIndividual ,
                          :Action .


###  http://www.semanticweb.org/danielhadad/AgriGame#TakeSheepAct
:TakeSheepAct rdf:type owl:NamedIndividual ,
                       :Action .


###  http://www.semanticweb.org/danielhadad/AgriGame#TakeStoneAct
:TakeStoneAct rdf:type owl:NamedIndividual ,
                       :Action .


###  http://www.semanticweb.org/danielhadad/AgriGame#TakeVegAct
:TakeVegAct rdf:type owl:NamedIndividual ,
                     :Action .


###  http://www.semanticweb.org/danielhadad/AgriGame#TakeWoodAct
:TakeWoodAct rdf:type owl:NamedIndividual ,
                      :Action .


###  http://www.semanticweb.org/danielhadad/AgriGame#UnfencedStable
:UnfencedStable rdf:type owl:NamedIndividual ,
                         :FarmyardSpace .


###  http://www.semanticweb.org/danielhadad/AgriGame#UnusedSpace
:UnusedSpace rdf:type owl:NamedIndividual ,
                      :FarmyardSpace .


###  http://www.semanticweb.org/danielhadad/AgriGame#UweActionBooster
:UweActionBooster rdf:type owl:NamedIndividual ,
                           :UweRevised .


###  http://www.semanticweb.org/danielhadad/AgriGame#UweBRProvider
:UweBRProvider rdf:type owl:NamedIndividual ,
                        :UweRevised .


###  http://www.semanticweb.org/danielhadad/AgriGame#UweCropProvider
:UweCropProvider rdf:type owl:NamedIndividual ,
                          :UweRevised .


###  http://www.semanticweb.org/danielhadad/AgriGame#UweFarmPlanner
:UweFarmPlanner rdf:type owl:NamedIndividual ,
                         :UweRevised .


###  http://www.semanticweb.org/danielhadad/AgriGame#UweFoodProvider
:UweFoodProvider rdf:type owl:NamedIndividual ,
                          :UweRevised .


###  http://www.semanticweb.org/danielhadad/AgriGame#UweGoodsProvider
:UweGoodsProvider rdf:type owl:NamedIndividual ,
                           :UweRevised .


###  http://www.semanticweb.org/danielhadad/AgriGame#UweLivestockProvider
:UweLivestockProvider rdf:type owl:NamedIndividual ,
                               :UweRevised .


###  http://www.semanticweb.org/danielhadad/AgriGame#UwePointsProvider
:UwePointsProvider rdf:type owl:NamedIndividual ,
                            :UweRevised .


###  http://www.semanticweb.org/danielhadad/AgriGame#VPGrp
:VPGrp rdf:type owl:NamedIndividual ,
                :Designation ;
       rdfs:comment "The category of cards that have the symbol for granting positive or negative Victory Points" .


###  http://www.semanticweb.org/danielhadad/AgriGame#Vegetable
:Vegetable rdf:type owl:NamedIndividual ,
                    :Crop .


###  http://www.semanticweb.org/danielhadad/AgriGame#WellGrp
:WellGrp rdf:type owl:NamedIndividual ,
                  :Designation ;
         rdfs:comment "Category of improvements that count as Wells" .


###  http://www.semanticweb.org/danielhadad/AgriGame#WildBoar
:WildBoar rdf:type owl:NamedIndividual ,
                   :Animal .


###  http://www.semanticweb.org/danielhadad/AgriGame#Wm
:Wm rdf:type owl:NamedIndividual ,
             :PublishedDeck ;
    rdfs:label "World Championship Deck" .


###  http://www.semanticweb.org/danielhadad/AgriGame#Wood
:Wood rdf:type owl:NamedIndividual ,
               :BuildingResource .


###  http://www.semanticweb.org/danielhadad/AgriGame#WoodHutRoom
:WoodHutRoom rdf:type owl:NamedIndividual ,
                      :Room .


###  http://www.semanticweb.org/danielhadad/AgriGame#WorkPhase
:WorkPhase rdf:type owl:NamedIndividual ,
                    :Phase ;
           rdfs:comment "The round phase in which players use action spaces by placing person and/or guest tokens. Ends when all players have placed all of their available person and guest tokens." .


###  http://www.semanticweb.org/danielhadad/AgriGame#1AnimalSpace
<http://www.semanticweb.org/danielhadad/AgriGame#1AnimalSpace> rdf:type owl:NamedIndividual ,
                                                                                          <http://www.semanticweb.org/danielhadad/AgriGame#5PlayerActionSpace> ;
                                                                                 rdfs:label "Take 1 Sheep and 1 Food or Take 1 Wild Boar or Pay 1 Food for 1 Cattle" .


###  http://www.semanticweb.org/danielhadad/AgriGame#1BoarSpace
<http://www.semanticweb.org/danielhadad/AgriGame#1BoarSpace> rdf:type owl:NamedIndividual ,
                                                                                        :Stage3ActionSpace ;
                                                                               rdfs:label "1 Wild Boar" .


###  http://www.semanticweb.org/danielhadad/AgriGame#1ClaySpace
<http://www.semanticweb.org/danielhadad/AgriGame#1ClaySpace> rdf:type owl:NamedIndividual ,
                                                                                        :BoardActionSpace ;
                                                                               rdfs:label "1 Clay" .


###  http://www.semanticweb.org/danielhadad/AgriGame#1CowSpace
<http://www.semanticweb.org/danielhadad/AgriGame#1CowSpace> rdf:type owl:NamedIndividual ,
                                                                                       :Stage4ActionSpace ;
                                                                              rdfs:label "1 Cattle" .


###  http://www.semanticweb.org/danielhadad/AgriGame#1ReedSpace
<http://www.semanticweb.org/danielhadad/AgriGame#1ReedSpace> rdf:type owl:NamedIndividual ,
                                                                                        :BoardActionSpace ;
                                                                               rdfs:label "1 Reed" .


###  http://www.semanticweb.org/danielhadad/AgriGame#1ReedStoneWoodSpace
<http://www.semanticweb.org/danielhadad/AgriGame#1ReedStoneWoodSpace> rdf:type owl:NamedIndividual ,
                                                                                                 <http://www.semanticweb.org/danielhadad/AgriGame#5PlayerActionSpace> ;
                                                                                        rdfs:label "1 Reed. In addition, take 1 Stone and 1 Wood" .


###  http://www.semanticweb.org/danielhadad/AgriGame#1ResourceSpace
<http://www.semanticweb.org/danielhadad/AgriGame#1ResourceSpace> rdf:type owl:NamedIndividual ,
                                                                                            <http://www.semanticweb.org/danielhadad/AgriGame#3PlayerActionSpace> ;
                                                                                   rdfs:label "Take 1 Building Resource of your choice" .


###  http://www.semanticweb.org/danielhadad/AgriGame#1RoomOrTPSpace
<http://www.semanticweb.org/danielhadad/AgriGame#1RoomOrTPSpace> rdf:type owl:NamedIndividual ,
                                                                                            <http://www.semanticweb.org/danielhadad/AgriGame#5PlayerActionSpace> ;
                                                                                   rdfs:label "Build 1 Room or Traveling Players" .


###  http://www.semanticweb.org/danielhadad/AgriGame#1SheepSpace
<http://www.semanticweb.org/danielhadad/AgriGame#1SheepSpace> rdf:type owl:NamedIndividual ,
                                                                                         :Stage1ActionSpace ;
                                                                                rdfs:label "1 Sheep" .


###  http://www.semanticweb.org/danielhadad/AgriGame#1StoneStage2Space
<http://www.semanticweb.org/danielhadad/AgriGame#1StoneStage2Space> rdf:type owl:NamedIndividual ,
                                                                                               :Stage2ActionSpace ;
                                                                                      rdfs:label "1 Stone" .


###  http://www.semanticweb.org/danielhadad/AgriGame#1StoneStage4Space
<http://www.semanticweb.org/danielhadad/AgriGame#1StoneStage4Space> rdf:type owl:NamedIndividual ,
                                                                                               :Stage4ActionSpace ;
                                                                                      rdfs:label "1 Stone" .


###  http://www.semanticweb.org/danielhadad/AgriGame#1WoodSpace
<http://www.semanticweb.org/danielhadad/AgriGame#1WoodSpace> rdf:type owl:NamedIndividual ,
                                                                                        <http://www.semanticweb.org/danielhadad/AgriGame#4PlayerActionSpace> ;
                                                                               rdfs:label "1 Wood" .


###  http://www.semanticweb.org/danielhadad/AgriGame#2ClaySpace
<http://www.semanticweb.org/danielhadad/AgriGame#2ClaySpace> rdf:type owl:NamedIndividual ,
                                                                                        <http://www.semanticweb.org/danielhadad/AgriGame#4PlayerActionSpace> ;
                                                                               rdfs:label "2 Clay" .


###  http://www.semanticweb.org/danielhadad/AgriGame#2Room
<http://www.semanticweb.org/danielhadad/AgriGame#2Room> rdf:type owl:NamedIndividual ,
                                                                                   :Strategy ;
                                                                          rdfs:comment "A strategic approach where the player does not build any additional rooms." .


###  http://www.semanticweb.org/danielhadad/AgriGame#2WoodSpace
<http://www.semanticweb.org/danielhadad/AgriGame#2WoodSpace> rdf:type owl:NamedIndividual ,
                                                                                        <http://www.semanticweb.org/danielhadad/AgriGame#4PlayerActionSpace> ;
                                                                               rdfs:label "2 Wood" .


###  http://www.semanticweb.org/danielhadad/AgriGame#3ClaySpace
<http://www.semanticweb.org/danielhadad/AgriGame#3ClaySpace> rdf:type owl:NamedIndividual ,
                                                                                        <http://www.semanticweb.org/danielhadad/AgriGame#5PlayerActionSpace> ;
                                                                               rdfs:label "3 Clay" .


###  http://www.semanticweb.org/danielhadad/AgriGame#3Player1ClaySpace
<http://www.semanticweb.org/danielhadad/AgriGame#3Player1ClaySpace> rdf:type owl:NamedIndividual ,
                                                                                               <http://www.semanticweb.org/danielhadad/AgriGame#3PlayerActionSpace> ;
                                                                                      rdfs:label "1 Clay" .


###  http://www.semanticweb.org/danielhadad/AgriGame#3Player2WoodSpace
<http://www.semanticweb.org/danielhadad/AgriGame#3Player2WoodSpace> rdf:type owl:NamedIndividual ,
                                                                                               <http://www.semanticweb.org/danielhadad/AgriGame#3PlayerActionSpace> ;
                                                                                      rdfs:label "2 Wood" .


###  http://www.semanticweb.org/danielhadad/AgriGame#3PlayerExpensiveOccSpace
<http://www.semanticweb.org/danielhadad/AgriGame#3PlayerExpensiveOccSpace> rdf:type owl:NamedIndividual ,
                                                                                                      <http://www.semanticweb.org/danielhadad/AgriGame#3PlayerActionSpace> ;
                                                                                             rdfs:comment "Costs 2 Food" ;
                                                                                             rdfs:label "1 Occupation" .


###  http://www.semanticweb.org/danielhadad/AgriGame#3Room
<http://www.semanticweb.org/danielhadad/AgriGame#3Room> rdf:type owl:NamedIndividual ,
                                                                                   :Strategy ;
                                                                          rdfs:comment "A strategic approach where the player aims to build exactly one additional room over the course of the game." .


###  http://www.semanticweb.org/danielhadad/AgriGame#3WoodSpace
<http://www.semanticweb.org/danielhadad/AgriGame#3WoodSpace> rdf:type owl:NamedIndividual ,
                                                                                        :BoardActionSpace ;
                                                                               rdfs:label "3 Wood" .


###  http://www.semanticweb.org/danielhadad/AgriGame#4WOcc
<http://www.semanticweb.org/danielhadad/AgriGame#4WOcc> rdf:type owl:NamedIndividual ,
                                                                                   :SimilarUse ;
                                                                          rdfs:comment "The category of cards that offer a diminishing number of building resources (usually wood) depending on the number of rounds left to play. Cards in this category offer global bonus points." .


###  http://www.semanticweb.org/danielhadad/AgriGame#4WoodSpace
<http://www.semanticweb.org/danielhadad/AgriGame#4WoodSpace> rdf:type owl:NamedIndividual ,
                                                                                        <http://www.semanticweb.org/danielhadad/AgriGame#5PlayerActionSpace> ;
                                                                               rdfs:label "4 Wood" .


#################################################################
#    General axioms
#################################################################

[ rdf:type owl:AllDisjointClasses ;
  owl:members ( :Designation
                :SimilarUse
                :Strategy
                :UweRevised
              )
] .


[ rdf:type owl:AllDisjointClasses ;
  owl:members ( :Stage1ActionSpace
                :Stage2ActionSpace
                :Stage3ActionSpace
                :Stage4ActionSpace
                :Stage5ActionSpace
                :Stage6ActionSpace
              )
] .


[ rdf:type owl:AllDisjointClasses ;
  owl:members ( <http://www.semanticweb.org/danielhadad/AgriGame#1PlusOccupation>
                <http://www.semanticweb.org/danielhadad/AgriGame#3PlusOccupation>
                <http://www.semanticweb.org/danielhadad/AgriGame#4PlusOccupation>
              )
] .


[ rdf:type owl:AllDisjointClasses ;
  owl:members ( <http://www.semanticweb.org/danielhadad/AgriGame#3PlayerActionSpace>
                <http://www.semanticweb.org/danielhadad/AgriGame#4PlayerActionSpace>
                <http://www.semanticweb.org/danielhadad/AgriGame#5PlayerActionSpace>
              )
] .


###  Generated by the OWL API (version 4.5.9.2019-02-01T07:24:44Z) https://github.com/owlcs/owlapi
